src/Framework/Simulation/Metatheory.v
@@ -3,17 +3,19 @@ Require Import Simulation.Definitions Simulation.WeakestPreconditions.
 
 Theorem transfer_high_to_low:
   forall OL OH (LL: Language OL) (LH: Language OH) (R: Refinement LL LH)
+    rec
     related_states_h
     valid_state_h
     valid_prog_h,
     
     SelfSimulation
       LH
+      rec
       valid_state_h
       valid_prog_h
       related_states_h ->
     
-    StrongBisimulation R ->
+    StrongBisimulation R rec ->
 
     high_oracle_exists R ->
     
@@ -21,35 +23,136 @@ Theorem transfer_high_to_low:
 
     exec_compiled_preserves_validity  R                           
     (refines_to_valid R valid_state_h) ->
+
+    (** All after_crash states_are valid **)
+    (forall sh,
+       valid_state_h sh ->
+       forall shc,
+         LH.(after_crash) sh shc ->
+         valid_state_h shc) ->
+
+    valid_prog_h _ rec ->
+
+    (forall sl sh slc,
+       R.(refines_to) sl sh ->
+       LL.(after_crash) sl slc ->
+       
+       exists shc,
+         LH.(after_crash) sh shc /\
+         R.(refines_to) slc shc) ->
+
+    (forall sl sh shc,
+       R.(refines_to) sl sh ->
+       LH.(after_crash) sh shc ->
+       
+       exists slc,
+         LL.(after_crash) sl slc /\
+         R.(refines_to) slc shc) ->
     
     SelfSimulation
       LL
+      (R.(compile) rec)
       (refines_to_valid R valid_state_h)
       (compiles_to_valid R valid_prog_h)
       (refines_to_related R related_states_h).
 Proof.
   unfold refines_to_related, compiles_to_valid; intros.
-  destruct H, H0.
   
-  eapply Build_SelfSimulation;  intros; cleanup.
-  match goal with
-  | [H: high_oracle_exists _,
-     H0: exec LL _ _ _ _ |- _] =>
-    edestruct H; try apply H0; eauto
-  end.
+  unfold SelfSimulation;  intros; cleanup.
+
+  Set Nested Proofs Allowed.
+  
+  Lemma high_oracle_exists_recovery_exec:
+    forall OL OH (LL: Language OL) (LH: Language OH) (R: Refinement LL LH)
+      T (p: prog LH T) rec o1 o2 s1 s1',
+
+      (exists sh, R.(refines_to) s1 sh) -> 
+      high_oracle_exists R  ->
+
+      exec_compiled_preserves_refinement R ->
+
+      (forall sl sh slc,
+       R.(refines_to) sl sh ->
+       LL.(after_crash) sl slc ->
+       
+       exists shc,
+         LH.(after_crash) sh shc /\
+         R.(refines_to) slc shc) ->
+    
+      recovery_exec LL o1 o2 s1 (compile R p) (compile R rec) s1' ->
+      (exists o1h,
+         R.(oracle_refines_to) s1 p o1 o1h) /\
+      (forall sc,
+         exec LL o1 s1 (compile R p) (Crashed sc) ->
+         exists sac o2h,
+           LL.(after_crash) sc sac /\
+           R.(oracle_refines_to) sac rec o2 o2h).
+  Proof.
+    intros; invert_exec.
+    {
+      edestruct H0; eauto.
+      split; eauto.
+      intros.
+      eapply exec_deterministic_wrt_oracle in H11; eauto; cleanup.
+    }
+    edestruct H0; eauto.
+    split; eauto.
+    intros.
+    eapply exec_deterministic_wrt_oracle in H6; eauto; cleanup.
+    eexists; intros.
+    edestruct H1; eauto; simpl in *.
+    edestruct H2; eauto; cleanup.
+    edestruct H0; try apply H13; eauto.
+  Qed.
+
+  eapply_fresh high_oracle_exists_recovery_exec in H10; eauto; cleanup.
   
   match goal with
-  | [H: refines_to _ s1 _ |- _] =>
-    eapply_fresh strong_bisimulation_correct in H; eauto; cleanup
+  | [H: oracle_refines_to _ s1 _ _ _,
+        H0: StrongBisimulation _ _ |- _] =>
+    eapply_fresh H0 in H; eauto; cleanup
   end.
 
-  match goal with
-    | [H: forall _, exec LL _ _ _ _ -> _,
-       H0: exec LL _ _ _ _,
-       H1: forall _, exec LH _ _ _ _ -> _ |- _] =>
-      eapply_fresh H in H0; cleanup; clear H H1
-  end.
+  Lemma oracle_refines_to_recovery_exec:
+    forall OL OH (LL: Language OL) (LH: Language OH) (R: Refinement LL LH)
+      T (p: prog LH T) rec o1 o1r s1 s1',
+    recovery_exec LL o1 o1r s1 (compile R p) (compile R rec) s1' ->
+    (forall sc : Language.state' OL,
+        exec LL o1 s1 (compile R p) (Crashed sc) ->
+        exists (sac : Operation.state OL) (o2h : oracle LH),
+          after_crash LL sc sac /\ oracle_refines_to R sac rec o1r o2h) ->
+    (forall (s1c : Language.state' OL) (s1r : Operation.state OL),
+        exec LL o1 s1 (compile R p) (Crashed s1c) ->
+        after_crash LL s1c s1r -> exists o2r, oracle_refines_to R s1r rec o1r o2r).
+  Proof.
+    intros; invert_exec;
+    eapply exec_deterministic_wrt_oracle in H1; eauto; cleanup.
+    eapply H0 in H5; cleanup.
+    
+  
+  {(** Finished **)
+    match goal with
+    | [H: high_oracle_exists _,
+          H0: Language.exec' _ _ _ _ |- _] =>
+      edestruct H; try apply H0; eauto
+    end.
+    
+    match goal with
+    | [H: oracle_refines_to _ s1 _ _ _,
+          H0: StrongBisimulation _ _ |- _] =>
+      eapply_fresh H0 in H; eauto; cleanup
+    end.
 
+    edestruct Hx; intros.
+    eapply exec_deterministic_wrt_oracle in H19; eauto; cleanup.
+   
+  match goal with
+    | [H: forall _, recovery_exec LL _ _ _ _ _ _ -> _,
+       H0: Language.exec' _ _ _ _,
+       H1: forall _, recovery_exec LH _ _ _ _ _ _ -> _ |- _] =>
+      edestruct H; [solve [econstructor; eauto] |];
+      cleanup; clear H H1; simpl in *
+  end.
 
   match goal with
   | [H: refines_to_valid _ _ ?s,
@@ -61,31 +164,170 @@ Proof.
   end.
 
   match goal with
-    | [H: exec LH _ _ _ _ |- _] =>
-      eapply_fresh self_simulation_correct in H; eauto; cleanup
+    [H: SelfSimulation LH _ _ _ _,
+        H0: recovery_exec LH _ _ _ _ _ _|- _] =>
+    eapply_fresh H in H0; eauto
   end.
+  match goal with
+      [H: related_states_h _ _ -> _,
+       H0: related_states_h _ _ |- _] =>
+      specialize H with (1:= H0); cleanup
+  end.
+
   
   match goal with
-  | [H: exec LH _ ?x2 _ _,
+  | [H: Language.exec' _ ?x2 _ _,
      H0: refines_to _ ?s1 ?x1,
      H1: refines_to _ ?s2 ?x2,      
-     H2: refines_to_valid _ _ ?s2 |- _] =>
-      eapply_fresh strong_bisimulation_correct in H1; eauto; cleanup
+     H2: refines_to_valid _ _ ?s2,
+     H3: StrongBisimulation _ |- _] =>
+      eapply_fresh H3 in H1; eauto; cleanup
   end.
-  
-  match goal with
-    | [H: forall _, exec LL _ _ _ _ -> _,
-       H0: exec LH _ _ _ _,
-       H1: forall _, exec LH _ _ _ _ -> _ |- _] =>
-      eapply_fresh H1 in H0; cleanup; clear H H1
-  end.  
-  
-  do 2 eexists; intuition eauto.
 
   match goal with
-  |[ H0: oracle_refines_to_same_from_related _ _ |- _] =>
-      eapply H0; eauto
+  |[ H: oracle_refines_to _ _ _ _ _,
+     H0: oracle_refines_to_same_from_related _ _ |- _] =>
+      eapply H0 in H; unfold refines_to_related; eauto
   end.
+
+  match goal with
+  |[ H: oracle_refines_to _ ?s _ _ _,
+     H0: oracle_refines_to _ ?s _ _ _ -> _ |- _] =>
+   specialize H0 with (1:= H); cleanup
+  end.
+    
+  match goal with
+    | [H: forall _, exec LL _ _ _ _ -> _,
+       H0: Language.exec' _ _ _ _,
+       H1: forall _, exec LH _ _ _ _ -> _ |- _] =>
+      unfold exec in *;
+      eapply_fresh H1 in H0;
+      cleanup; clear H H1
+  end.  
+  
+  eexists; intuition eauto.
+  econstructor; eauto.
+
+  do 2 eexists; intuition eauto.
+  simpl; eauto.
+  unfold refines_to_valid; intuition eauto.
+  eapply X; unfold exec; try apply H19; eauto;
+  simpl; eauto.
+  simpl;
+  unfold refines_to_valid; intuition eauto.
+  eapply X; eauto.
+  }
+
+  { (** Recovered **)
+    simpl; eauto.
+     match goal with
+    | [H: high_oracle_exists _,
+          H0: Language.exec' _ _ _ (Crashed _) |- _] =>
+      edestruct H; try apply H0; eauto
+    end.
+    
+     match goal with
+     | [H: oracle_refines_to _ s1 _ _ _,
+          H0: StrongBisimulation _ |- _] =>
+      eapply_fresh H0 in H; eauto; cleanup
+    end.
+
+     match goal with
+     | [H: forall _, exec LL _ _ _ _ -> _,
+          H0: Language.exec' _ _ _ _,
+          H1: forall _, exec LH _ _ _ _ -> _ |- _] =>
+       eapply_fresh H in H0; cleanup; clear H H1
+     end.
+
+
+     match goal with
+     | [H: refines_to_valid _ _ ?s,
+           H0: refines_to _ ?s _,
+               H1: refines_to_valid _ _ ?t,
+                   H2: refines_to _ ?t _ |- _] =>
+       eapply_fresh H in H0;
+       eapply_fresh H1 in H2; cleanup
+     end.
+
+     match goal with
+     | [H: forall _ , after_crash _ _ _ -> _,
+          H0: Operation.after_crash _ _ _ |- _] =>
+       eapply_fresh H in H0; cleanup
+     end.
+     
+     match goal with
+     | [H: high_oracle_exists _,
+           H0: Language.exec' _ _ _ (Finished _ _) |- _] =>
+       edestruct H; try apply H0; eauto
+     end.
+     
+     match goal with
+     | [H: oracle_refines_to _ d_ac _ _ _,
+           H0: StrongBisimulation _ |- _] =>
+       eapply_fresh H0 in H; eauto; cleanup
+     end.
+
+     match goal with
+     | [H: forall _, exec LL _ _ _ _ -> _,
+          H0: Language.exec' _ _ _ _,
+          H1: forall _, exec LH _ _ _ _ -> _ |- _] =>
+       eapply_fresh H in H0; cleanup; clear H H1
+     end.
+
+     match goal with
+       [H: SelfSimulation LH _ _ _ _ |- _] =>
+       edestruct H; cleanup; try solve [
+       eapply ExecRecover; eauto]; eauto
+     end.
+
+     simpl in *; cleanup.
+     
+     match goal with
+     | [H: recovery_exec _ _ _ _ _ _ _ |- _] =>
+       inversion H; cleanup; clear H
+     end; simpl in *; cleanup.
+
+     
+     
+     match goal with
+     | [H: Language.exec' _ ?x2 _ _,
+           H3: StrongBisimulation _ |- _] =>
+       eapply_fresh H3 in H; cleanup
+     end.
+     
+
+     match goal with
+  |[ H: oracle_refines_to _ _ _ _ _,
+     H0: oracle_refines_to_same_from_related _ _ |- _] =>
+      eapply H0 in H; unfold refines_to_related; eauto
+  end.
+  
+  specialize Hx1 with (1:= H18); cleanup.
+  
+  match goal with
+    | [H: forall _, exec (LL _ _) _ _ _ _ -> _,
+       H0: Language.exec' _ _  _,
+       H1: forall _, exec (LH _ _) _ _ _ _ -> _ |- _] =>
+      unfold exec in *;
+      eapply_fresh H1 in H0;
+      cleanup; clear H H1
+  end.  
+  
+  eexists; intuition eauto.
+  econstructor; eauto.
+
+  do 2 eexists; intuition eauto.
+  simpl; eauto.
+  unfold refines_to_valid; intuition eauto.
+  eapply X; unfold exec; try apply H17; eauto;
+  simpl; eauto.
+  simpl;
+  unfold refines_to_valid; intuition eauto.
+  eapply X; eauto.
+  match goal with
+   
+
+  end
   unfold refines_to_related; eauto. 
 Qed.
 
