src/Layers/BasicLayers/Authentication/AuthenticationLayer.v
@@ -14,6 +14,9 @@ Set Implicit Arguments.
   Definition oracle' := list token'.  
 
   Definition state' := user.
+
+  (** TODO: This may need to change **)
+  Definition after_crash' (s1 s2: state') := s1 = s2.
   
   Inductive authentication_prog : Type -> Type :=
   | Auth : user -> authentication_prog (option unit).
@@ -129,6 +132,7 @@ Set Implicit Arguments.
   Definition AuthenticationOperation :=
     Build_Operation
       (list_eq_dec token_dec')
+      after_crash'
       authentication_prog
       exec'
       weakest_precondition'
@@ -142,6 +146,5 @@ Set Implicit Arguments.
       exec_deterministic_wrt_oracle'.
 
   Definition AuthenticationLang := Build_Language AuthenticationOperation.
-  Definition AuthenticationHL := Build_HoareLogic AuthenticationLang.
 
   Notation "p >> s" := (p s) (right associativity, at level 60, only parsing).
