src/Layers/ComposedLayers/AuthenticatedDisk/AuthenticatedDiskLayer.v
@@ -6,7 +6,6 @@ Set Implicit Arguments.
 
 Definition AuthenticatedDiskOperation :=  HorizontalComposition AuthenticationOperation (TransactionalDiskOperation data_length).
 Definition AuthenticatedDiskLang := Build_Language AuthenticatedDiskOperation.
-Definition AuthenticatedDiskHL := Build_HoareLogic AuthenticatedDiskLang.
 
 Notation "'|ADAP|' p" := (@lift_L1 AuthenticationOperation (TransactionalDiskOperation data_length) AuthenticationLang _ p) (at level 59).
 Notation "'|ADDP|' p" := (@lift_L2 AuthenticationOperation (TransactionalDiskOperation data_length) (TransactionalDiskLang data_length) _ p) (at level 59).
