src/Layers/ComposedLayers/CachedDisk/CachedDiskLayer.v
@@ -6,7 +6,6 @@ Set Implicit Arguments.
 
 Definition CachedDiskOperation :=  HorizontalComposition (CacheOperation addr_dec value) CryptoDiskOperation.
 Definition CachedDiskLang := Build_Language CachedDiskOperation.
-Definition CachedDiskHL := Build_HoareLogic CachedDiskLang.
 
 Notation "'|CDCP|' p" := (@lift_L1 (CacheOperation addr_dec value) CryptoDiskOperation (CacheLang addr_dec value) _ p) (at level 59).
 Notation "'|CDDP|' p" := (@lift_L2 (CacheOperation addr_dec value) CryptoDiskOperation CryptoDiskLang _ p) (at level 59).
