src/Refinements/FileToFileDisk/Refinement.v
@@ -1,12 +1,13 @@
 Require Import Framework FSParameters AuthenticatedDiskLayer FileDiskLayer.
 Require Import File FileToFileDisk.Definitions.
-Require Import ClassicalFacts FunctionalExtensionality Omega.
+Require Import ClassicalFacts FunctionalExtensionality Psatz.
+Require Import Arith.
 
 Set Nested Proofs Allowed.
 
-Notation "'low_op'" := TransactionalDiskOperation.
+Notation "'low_op'" := (TransactionalDiskOperation data_length).
 Notation "'high_op'" := (FileDiskOperation inode_count).
-Notation "'low'" := TransactionalDiskLang.
+Notation "'low'" := (TransactionalDiskLang data_length).
 Notation "'high'" := (FileDiskLang inode_count).
 Notation "'refinement'" := FileDiskRefinement.
 
@@ -28,22 +29,22 @@ Section FileDiskBisimulation.
       j < length l ->
       nth i l def1 <> nth j l def2.
   Proof.
-    induction l; simpl; intros; try omega.
-    destruct i, j; try omega.
+    induction l; simpl; intros; try lia.
+    destruct i, j; try lia.
     inversion H; cleanup.
     intros Heq.
     apply H5.
     rewrite Heq.
-    eapply nth_In; omega.
+    eapply nth_In; lia.
 
     inversion H; cleanup.
     intros Heq.
     apply H5.
     rewrite <- Heq.
-    eapply nth_In; omega.
+    eapply nth_In; lia.
 
     inversion H; cleanup.
-    eapply IHl; eauto; omega.
+    eapply IHl; eauto; lia.
   Qed.
 
   Lemma NoDup_app_nth_ne:
@@ -53,18 +54,18 @@ Section FileDiskBisimulation.
       j < length l2 ->
       nth i l1 def1 <> nth j l2 def2.
   Proof.
-    induction l1; simpl; intros; try omega.
-    destruct i; try omega.
+    induction l1; simpl; intros; try lia.
+    destruct i; try lia.
     inversion H; cleanup.
     intros Heq.
     apply H4.
     rewrite Heq.
     apply in_or_app.
     right.
-    eapply nth_In; omega.
+    eapply nth_In; lia.
 
-    destruct l2; simpl in *; try omega.
-    destruct j; try omega.
+    destruct l2; simpl in *; try lia.
+    destruct j; try lia.
     inversion H; cleanup.
     intros Heq.
 
@@ -74,13 +75,13 @@ Section FileDiskBisimulation.
     apply H6.
     apply in_or_app.
     right.
-    eapply nth_In; omega.
+    eapply nth_In; lia.
 
     inversion H; cleanup.
     apply NoDup_app_comm in H5.
     simpl in *.
     inversion H5; cleanup.
-    eapply IHl1; eauto; try omega.
+    eapply IHl1; eauto; try lia.
     apply NoDup_app_comm; eauto.
   Qed.
   
@@ -100,7 +101,7 @@ Section FileDiskBisimulation.
     unfold files_inner_rep; intros; cleanup.
     destruct (lt_dec a0 (length (blocks f))).
     2: {
-      rewrite updN_oob by omega.
+      rewrite updN_oob by lia.
       destruct f; simpl in *;
       rewrite upd_nop; eauto.
     }              
@@ -131,7 +132,7 @@ Section FileDiskBisimulation.
       erewrite nth_error_nth'.
       rewrite <- nth_selN_eq.
       rewrite selN_updN_eq_default; eauto.
-      rewrite length_updN; omega.
+      rewrite length_updN; lia.
       rename H8 into Hx.
       erewrite nth_error_nth' in Hx; cleanup; eauto.
       
@@ -144,12 +145,12 @@ Section FileDiskBisimulation.
       rename H8 into Hx.
       apply some_not_none in Hx.
       apply nth_error_Some in Hx.
-      omega.
+      lia.
       
       rename H8 into Hx.
       apply some_not_none in Hx.
       apply nth_error_Some in Hx.
-      rewrite length_updN; omega.
+      rewrite length_updN; lia.
       assert (Alen: i < length (Inode.block_numbers inode)).
       {
         eapply nth_error_Some; congruence.
@@ -183,6 +184,7 @@ Section FileDiskBisimulation.
     }
   Qed.
 
+  (*
   Lemma refines_to_upd:
     forall s1 s2 a a0 f v,
       refines_to s1 s2 ->
@@ -196,17 +198,19 @@ Section FileDiskBisimulation.
     unfold refines_to; simpl; intros; cleanup.
     destruct (lt_dec a0 (length (blocks f))).
     2: {
-      rewrite updN_oob by omega.
+      rewrite updN_oob by lia.
       destruct f; simpl in *;
       rewrite upd_nop; eauto.
     }
     
-    unfold files_rep in *.
-    destruct H1 as [imap Hx].
+    unfold files_rep in *.    
+    apply pimpl_exists_l_star_r in H2.
+    destruct H2 as [imap Hx].
+    rewrite pimpl_exists_l_star_r in Hx.
     apply pimpl_exists_l_star_r in Hx.
     destruct Hx as [fbmap Hx].
     destruct_lift Hx.
-    eapply files_inner_rep_upd in H5; eauto.
+    eapply files_inner_rep_upd in H7; eauto.
     cleanup.
     exists (fst s2, (upd (fst (snd s1)) a0 v, snd (snd s1))).
     simpl; intuition eauto.        
@@ -221,7 +225,7 @@ Section FileDiskBisimulation.
     Unshelve.
     all: eauto.
   Admitted.
-
+   *)
   Lemma files_inner_rep_extend:
     forall fmap imap fbmap a v f bn,
       files_inner_rep fmap imap fbmap ->
@@ -269,18 +273,18 @@ Section FileDiskBisimulation.
       rewrite Nat.add_1_r in Hx.
       inversion Hx; subst.
       {
-        rewrite nth_error_app2; try omega.
+        rewrite nth_error_app2; try lia.
         rename H9 into Hy.
-        rewrite nth_error_app2 in Hy; try omega.
+        rewrite nth_error_app2 in Hy; try lia.
         rewrite Nat.sub_diag in Hy.
         rewrite H7, Nat.sub_diag;
         simpl in *; cleanup.
         rewrite upd_eq; eauto.
       }
       {
-        rewrite nth_error_app1; try omega.
+        rewrite nth_error_app1; try lia.
         rename H9 into Hy.
-        rewrite nth_error_app1 in Hy; try omega.
+        rewrite nth_error_app1 in Hy; try lia.
         rewrite upd_ne; eauto.
 
         rename H0 into Hfree.
@@ -401,7 +405,7 @@ Section FileDiskBisimulation.
     eapply not_In_NoDup_app; eauto.
   Qed.
   
-
+  (*
   Lemma refines_to_extend:
     forall s1 s2 a f v,
       refines_to s1 s2 ->
@@ -571,9 +575,36 @@ Section FileDiskBisimulation.
       eapply refines_to_delete; eauto.
     }
   Qed.
-  
-  Axiom exec_compiled_preserves_refinement:
+ 
+   
+  Theorem exec_compiled_preserves_refinement:
     exec_compiled_preserves_refinement refinement.
+  Proof.
+    unfold exec_compiled_preserves_refinement.
+    induction p2; simpl; intros; cleanup.
+    { (** Op p **)
+      destruct p; simpl in *.
+      { (** read **)
+        destruct ret; simpl in *.
+        { (** Finished **)
+          eapply exec_to_sp with (P:= fun o s => refines_to s x /\ s = s1 /\ o = o1) in H0; eauto.
+          eapply sp_impl in H0.
+          apply read_ok in H0; unfold refines_to in *;
+          simpl; intros; eauto.
+          cleanup.
+          split_ors; cleanup.
+
+          exists (fst s, snd x); intuition eauto.
+          simpl; cleanup.
+          setoid_rewrite H2.
+          rewrite mem_union_empty_mem.
+          pred_apply' H2; cancel.
+          instantiate (1:= emp).
+          cancel.
+          split_ors; cleanup.
+          destruct s1; simpl in *.
+          repeat (simpl in *; cleanup).
+Admitted.          
 
   Theorem exec_preserves_refinement:
     exec_preserves_refinement refinement.
@@ -590,7 +621,7 @@ Section FileDiskBisimulation.
         eapply scp_implies_refines_to; eauto;
         eapply exec_to_scp; eauto.
       }
-    }
+      }
     { (* Ret *)
       cleanup; invert_exec; cleanup; simpl; eauto.
     }
@@ -605,993 +636,936 @@ Section FileDiskBisimulation.
         edestruct IHp; eauto;
         edestruct H; eauto.
       }
-    }
+      }
   Qed.
-  
-  
-  
-  (*
-
-            Lemma merge_some_l:
-              forall AT AEQ V (m1: @mem AT AEQ V) m2 a v,
-                m1 a = Some v ->
-                merge m1 m2 a = Some v.
-            Proof.
-              unfold merge; simpl; intros.
-              cleanup; eauto.
-            Qed.
-            
-            Lemma merge_some_r:
-              forall AT AEQ V (m1: @mem AT AEQ V) m2 a,
-                m1 a = None ->
-                merge m1 m2 a = m2 a.
-            Proof.
-              unfold merge; simpl; intros.
-              cleanup; eauto.
-            Qed.
    *)
-
-  Lemma apply_list_app:
-    forall A AEQ V  l l' (m: @mem A AEQ V), 
-      apply_list m (l++l') =
-      apply_list (apply_list m l) l'.
-  Proof.
-    induction l; simpl; eauto.
-  Qed.
   
   Lemma wp_low_to_high_read :
     forall inum a,
-      wp_low_to_high_prog' _ _ _ _ refinement _ (|Read inum a|).
+      wp_low_to_high_prog' _ _ _ _ refinement _ (Op high_op (Read inum a)).
+  Proof.
+    unfold wp_low_to_high_prog'; intros; cleanup.
+    eapply wp_to_exec in H; cleanup.
+    simpl in H1; cleanup.
+    eapply exec_deterministic_wrt_oracle in H; eauto; cleanup.
+    destruct H4; cleanup.    
+    split_ors; cleanup;
+    eapply exec_deterministic_wrt_oracle in H1; eauto; cleanup.
+    
+    simpl in *.
+    eexists; intuition eauto.
+    eapply exec_to_sp with (P := fun o s => refines_to s s2 /\ s = s1 /\ o = o1) in H2; eauto.
+
+    unfold refines_to in H0; cleanup.
+
+    eapply sp_impl in H2.
+    eapply read_ok in H2.
+
+    split_ors; cleanup.
+    {
+      destruct_fresh (nth_error (blocks x0) a).
+      {
+        left; intuition eauto.
+        (** TODO: Solve this from file existence. **)
+        admit.
+        do 2 eexists; intuition eauto.
+        unfold refines_to in *; cleanup; eauto.
+      }
+      {
+        right; intuition eauto.
+        unfold refines_to; intuition eauto.
+      }
+    }
+
+    {
+      right; intuition eauto.      
+      unfold refines_to in *; cleanup; eauto.
+      unfold refines_to in *; cleanup; eauto.
+      right; right;
+      eexists; intuition eauto.
+      unfold refines_to in *; cleanup; eauto.
+    }
+    simpl; intros.
+    cleanup; eauto.
+  Admitted.
+  
+  Lemma wp_high_to_low_read :
+    forall inum a,
+      wp_high_to_low_prog' _ _ _ _ refinement _ (Op high_op (Read inum a)).
+  Proof.
+    unfold wp_high_to_low_prog'; intros; cleanup.
+    simpl in H; cleanup.
+    repeat invert_exec; cleanup.
+    {
+      simpl in H1; cleanup.
+      destruct H1; cleanup.
+      split_ors; cleanup.
+      eapply exec_to_wp; eauto; simpl.
+      split; eauto.
+      split_ors; cleanup; try lia.
+      
+      eapply exec_to_sp with (P := fun o s => refines_to s s2' /\ o = o1 /\ s = s1) in H1; eauto.
+      unfold refines_to in H1.
+      apply sp_extract_precondition in H1; cleanup.
+      eapply sp_impl in H1.
+      eapply read_ok in H1.
+      split_ors; cleanup.
+      instantiate (1:= snd s2') in H1; cleanup; eauto.
+      split_ors; cleanup.
+      simpl in *; unfold refines_to in *; cleanup; exfalso; eauto.
+
+      clear H1.
+      simpl in *; intros; cleanup; eauto.
+    }
+    {
+      destruct H3; cleanup; try lia.
+      simpl in H1; cleanup.
+      destruct H1; cleanup.
+      destruct H1; cleanup.
+      eapply exec_to_wp; eauto; simpl.
+      split; eauto.
+      
+      eapply exec_to_sp with (P := fun o s => refines_to s s2' /\ o = o1 /\ s = s1) in H1; eauto.
+      unfold refines_to in H1.
+      apply sp_extract_precondition in H1; cleanup.
+      eapply sp_impl in H1.
+      eapply read_ok in H1.
+      destruct H1; cleanup; eauto.
+      
+      (** TODO: contradict with file existing **)
+      admit.
+
+      clear H1 H2 H7.
+      simpl in *; intros; cleanup; eauto.
+    }    
+  Admitted.
+
+  Lemma wcp_low_to_high_read :
+    forall inum a,
+      wcp_low_to_high_prog' _ _ _ _ refinement _ (Op high_op (Read inum a)).
+  Proof.
+    unfold wcp_low_to_high_prog'; intros; cleanup.
+    eapply wcp_to_exec in H; cleanup.
+    simpl in H1; cleanup.
+    eapply exec_deterministic_wrt_oracle in H; eauto; cleanup.
+    destruct H4; cleanup.    
+    split_ors; cleanup;
+    eapply exec_deterministic_wrt_oracle in H1; eauto; cleanup.
+    
+    simpl in *.
+    eexists; intuition eauto.
+  Qed.
+  
+  Lemma wcp_high_to_low_read :
+    forall inum a,
+      wcp_high_to_low_prog' _ _ _ _ refinement _ (Op high_op (Read inum a)).
+  Proof.
+    unfold wcp_high_to_low_prog'; intros; cleanup.
+    simpl in H; cleanup.
+    repeat invert_exec; cleanup.
+    simpl in H1; cleanup.
+    destruct H1; cleanup.
+    split_ors; cleanup.
+    eapply exec_to_wcp; eauto.
+  Qed.
+  
+  Lemma wp_low_to_high_write :
+    forall inum a v,
+      wp_low_to_high_prog' _ _ _ _ refinement _ (Op high_op (Write inum a v)).
   Proof.
     unfold wp_low_to_high_prog'; intros; cleanup.
     simpl in H1; cleanup.
-    destruct H3; cleanup.    
-    split_ors; cleanup; eapply exec_deterministic_wrt_oracle in H3; eauto; cleanup.
-    
-    eapply wp_to_exec in H; cleanup.
-    eapply exec_deterministic_wrt_oracle in H; eauto; cleanup.
-    simpl in *.
+    destruct H3; cleanup.
+    repeat (split_ors; cleanup); eapply exec_deterministic_wrt_oracle in H3; eauto; cleanup.
+    eapply exec_to_sp with (P := fun o s => refines_to s s2 /\ o = o1 /\ s = s1) in H2; eauto.
+    unfold write in *.
+    simpl; cleanup.
     eexists; intuition eauto.
-    eapply exec_to_sp with (P := fun o s => refines_to s s2 /\ s = x) in H2; eauto.
+    left; intuition eauto.
     
-    repeat (cleanup; simpl in *);
-            try match goal with
-                | [H: strongest_postcondition _ _ _ _ _ |- _] =>
-                  inversion H; clear H; cleanup
-                end;
+    clear H1 H17; unfold refines_to in *; simpl in *; cleanup.
+    rewrite apply_list_app; eauto.
+  Qed.
+  
+  Lemma wp_high_to_low_write :
+    forall a vl,
+      wp_high_to_low_prog' _ _ _ _ refinement _ (|Write a vl|).
+  Proof.
+    unfold wp_high_to_low_prog', compilation_of; simpl; intros; cleanup.
+    unfold compilation_of in *; simpl; intros; cleanup.
+    repeat invert_exec; cleanup.
+    repeat (split_ors; cleanup).
+    eapply exec_to_wp; simpl; eauto.
+    eapply exec_to_sp with (P := fun o s => refines_to s s2) in H; eauto.
+    unfold write in *.
+    simpl in *; cleanup.
+    eexists; intuition eauto.
+    clear H1; unfold refines_to in *; simpl in *; cleanup.
+    rewrite apply_list_app; eauto.
+    rewrite <- H1 at 1; rewrite apply_list_app; simpl; eauto.
+  Qed.
+  
+  
+  Lemma wcp_low_to_high_write :
+    forall a vl,
+      wcp_low_to_high_prog' _ _ _ _ refinement _ (|Write a vl|).
+  Proof.
+    unfold wcp_low_to_high_prog', compilation_of; simpl; intros; cleanup.
+    unfold compilation_of in *; simpl; intros; cleanup.
+    split_ors; cleanup; eapply exec_deterministic_wrt_oracle in H0; eauto; cleanup.
+    split_ors; cleanup;
+    eexists; intuition eauto.
+    
+    right; intuition eauto.
+    apply refines_to_upd; eauto.
+  Qed.
+  
+  Lemma wcp_high_to_low_write :
+    forall a vl,
+      wcp_high_to_low_prog' _ _ _ _ refinement _ (|Write a vl|).
+  Proof.
+    unfold wcp_high_to_low_prog', compilation_of; simpl; intros; cleanup.
+    unfold compilation_of in *; simpl; intros; cleanup.
+    repeat split_ors; cleanup; repeat invert_exec;
+    try inversion H8; try clear H8; cleanup;
+    try inversion H9; try clear H9; cleanup;
+    eapply exec_to_wcp; eauto.
+    - split_ors; cleanup; eauto.
+      
+    - split_ors; cleanup; eauto.
+      repeat invert_exec;
+      repeat match goal with
+             | [H: Operation.exec _ _ _ _ _ |- _ ] =>
+               inversion H; clear H; cleanup
+             | [H: exec' _ _ _ _ |- _ ] =>
+               inversion H; clear H; cleanup
+             end.
+      eapply refines_to_upd; eauto.
+  Qed.
+  
+  Lemma wp_low_to_high_start :
+    wp_low_to_high_prog' _ _ _ _ refinement _ (|Start|).
+  Proof.
+    unfold wp_low_to_high_prog', compilation_of; simpl; intros; cleanup.
+    unfold compilation_of in *; simpl in *; intros; cleanup.
+    split_ors; cleanup; eapply exec_deterministic_wrt_oracle in H0; eauto; cleanup.
+    eapply exec_to_sp with (P := fun o s => refines_to s s2) in H3; eauto.
+    simpl in *; cleanup.
+    eexists; intuition eauto.
+    clear H0 H9.
+    unfold refines_to in *; cleanup; eauto.
+  Qed.
 
-            unfold DiskAllocator.read in *; simpl in *;
-            repeat (cleanup; simpl in *);
-                    repeat (split_ors; cleanup;
-                            try match goal with
-                                | [H: strongest_postcondition _ _ _ _ _ |- _] =>
-                                  inversion H; clear H; cleanup
-                                end).
-                    
+  Lemma wp_high_to_low_start :
+    wp_high_to_low_prog' _ _ _ _ refinement _ (|Start|).
+  Proof.
+    unfold wp_high_to_low_prog', compilation_of; simpl; intros; cleanup.
+    unfold compilation_of in *; simpl; intros; cleanup.
+    repeat (split_ors; cleanup).
 
-                    
-                    - cleanup; eauto;
-                      try match goal with
-                          | [H: strongest_postcondition _ _ _ _ _ |- _] =>
-                            inversion H; clear H; cleanup
-                          end;
-                      cleanup.
+    repeat invert_exec; cleanup.    
+    eapply exec_to_wp; eauto.
+    eapply exec_to_sp with (P := fun o s => refines_to s s2) in H; eauto.
+    simpl in *; cleanup.
+    eexists; intuition eauto.
+    clear H H5.
+    unfold refines_to in *; cleanup; eauto.
+  Qed.
 
+  Lemma wcp_low_to_high_start :
+    wcp_low_to_high_prog' _ _ _ _ refinement _ (|Start|).
+  Proof.
+    unfold wcp_low_to_high_prog', compilation_of; simpl; intros; cleanup.
+    unfold compilation_of in *; simpl in *; intros; cleanup.
+    split_ors; cleanup; eapply exec_deterministic_wrt_oracle in H0; eauto; cleanup.
+    split_ors; cleanup; eauto.
+    eexists; intuition eauto.
+    right; unfold refines_to in *; cleanup; eauto.
+  Qed.
 
-                      unfold Inode.InodeAllocator.read in *; simpl in *.
-                      repeat (cleanup; simpl in *);
-                              repeat (split_ors; cleanup;
-                                      try match goal with
-                                          | [H: strongest_postcondition _ _ _ _ _ |- _] =>
-                                            inversion H; clear H; cleanup
-                                          end);
-                              
-                              try solve [ cleanup; simpl in *;
-                                          repeat cleanup;
-                                          repeat (split_ors; cleanup);
-                                          unfold empty_mem in *; simpl in *; congruence];
+  Lemma wcp_high_to_low_start :
+    wcp_high_to_low_prog' _ _ _ _ refinement _ (|Start|).
+  Proof.
+    unfold wcp_high_to_low_prog', compilation_of; simpl; intros; cleanup.
+    unfold compilation_of in *; simpl in *; intros; cleanup.
+    split_ors; cleanup.
+    repeat invert_exec.
+    eapply exec_to_wcp; eauto.
+    split_ors; cleanup.
+    repeat invert_exec; eauto.
+    repeat invert_exec; eauto.
+    cleanup.
+    repeat
+      match goal with
+      | [H: Operation.exec _ _ _ _ _ |- _ ] =>
+        inversion H; clear H; cleanup
+      | [H: exec' _ _ _ _ |- _ ] =>
+        inversion H; clear H; cleanup
+      end.
+    unfold refines_to in *; cleanup; eauto.
+  Qed.
 
-                              cleanup; simpl in *;
-                              repeat cleanup;
-                              repeat (split_ors; cleanup);
-                              repeat match goal with
-                                     | [H: strongest_postcondition _ _ _ _ _ |- _] =>
-                                       inversion H; clear H; cleanup
-                                     end;
-                              try solve [unfold empty_mem in *; simpl in *; congruence];
+  
+  Lemma wp_low_to_high_abort :
+    wp_low_to_high_prog' _ _ _ _ refinement _ (|Abort|).
+  Proof.
+    unfold wp_low_to_high_prog', compilation_of; simpl; intros; cleanup.
+    unfold compilation_of in *; simpl in *; intros; cleanup.
+    split_ors; cleanup; eapply exec_deterministic_wrt_oracle in H0; eauto; cleanup.
+    eapply exec_to_sp with (P := fun o s => refines_to s s2) in H3; eauto.
+    simpl in *; cleanup.
+    eexists; intuition eauto.
+    clear H1 H9.
+    unfold refines_to in *; simpl in *; cleanup; eauto.
+  Qed.
 
-                              try destruct x6; simpl in *; cleanup;
+  Lemma wp_high_to_low_abort :
+    wp_high_to_low_prog' _ _ _ _ refinement _ (|Abort|).
+  Proof.
+    unfold wp_high_to_low_prog', compilation_of; simpl; intros; cleanup.
+    unfold compilation_of in *; simpl; intros; cleanup.
+    repeat (split_ors; cleanup).
 
-                              repeat (split_ors; cleanup);
-                              repeat match goal with
-                                     | [H: strongest_postcondition _ _ _ _ _ |- _] =>
-                                       inversion H; clear H; cleanup
-                                     end;
-                              try solve [unfold empty_mem in *; simpl in *; congruence].
-                              
-                              +
+    repeat invert_exec; cleanup.    
+    eapply exec_to_wp; eauto.
+    eapply exec_to_sp with (P := fun o s => refines_to s s2) in H; eauto.
+    simpl in *; cleanup.
+    eexists; intuition eauto.
+    clear H1 H5.
+    unfold refines_to in *; simpl; cleanup; eauto.
+  Qed.
 
-                                match goal with
-                                | [H: strongest_postcondition _ _ _ _ _ |- _] =>
-                                  inversion H; clear H; cleanup
-                                end.
-                                try solve [unfold empty_mem in *; simpl in *; congruence].
-                                
-                                repeat (split_ors; cleanup);
-                                simpl in *.
-                                
-                                repeat (split_ors; cleanup;
-                                        try match goal with
-                                            | [H: strongest_postcondition _ _ _ _ _ |- _] =>
-                                              inversion H; clear H; cleanup
-                                            end).
-                                repeat cleanup.
-                                eexists; intuition eauto; unfold refines_to in *; cleanup;
-                                try congruence.      
-                                rewrite apply_list_get_latest_eq in D0; eauto.
-                                right; intuition.        
-                                rewrite <- apply_list_get_latest_eq; eauto.
-                               }
-                             cleanup; eauto.
-                              cleanup; simpl in *; cleanup.
-                              Qed.
+  Lemma wcp_low_to_high_abort :
+    wcp_low_to_high_prog' _ _ _ _ refinement _ (|Abort|).
+  Proof.
+    unfold wcp_low_to_high_prog', compilation_of; simpl; intros; cleanup.
+    unfold compilation_of in *; simpl in *; intros; cleanup.
+    split_ors; cleanup; eapply exec_deterministic_wrt_oracle in H0; eauto; cleanup.
+    split_ors; cleanup; eauto.
+    eexists; intuition eauto.
+    right; unfold refines_to in *; cleanup; eauto.
+  Qed.
 
-                              Lemma wp_high_to_low_read :
-                                forall a,
-                                  wp_high_to_low_prog' _ _ _ _ refinement _ (|Read a|).
-                              Proof.
-                                unfold wp_high_to_low_prog', compilation_of; simpl; intros; cleanup.
-                                unfold compilation_of in *; simpl; intros.
-                                simpl in *; subst.
-                                destruct H2; try solve [cleanup; split_ors; cleanup ].
-                                cleanup.
-                                repeat invert_exec.
-                                cleanup.
-                                eapply exec_to_wp; eauto; simpl.
-                                split; eauto.
-                                eapply exec_to_sp with (P := fun o s => refines_to s s2') in H; eauto.
-                                unfold read in *; simpl in *.
-                                cleanup; simpl in *.        
-                                rewrite apply_list_get_latest_eq in H; cleanup; simpl in *; cleanup;
-                                unfold refines_to in H; simpl in *; cleanup;    
-                                repeat split_ors; cleanup; eauto;
-                                try setoid_rewrite H2 in D; cleanup; eauto.
-                                try setoid_rewrite H3 in D; cleanup; eauto.
-                              Qed.
+  Lemma wcp_high_to_low_abort :
+    wcp_high_to_low_prog' _ _ _ _ refinement _ (|Abort|).
+  Proof.
+    unfold wcp_high_to_low_prog', compilation_of; simpl; intros; cleanup.
+    unfold compilation_of in *; simpl in *; intros; cleanup.
+    split_ors; cleanup.
+    repeat invert_exec.
+    eapply exec_to_wcp; eauto.
+    split_ors; cleanup.
+    repeat invert_exec; eauto.
+    repeat invert_exec; eauto.
+    cleanup.
+    repeat
+      match goal with
+      | [H: Operation.exec _ _ _ _ _ |- _ ] =>
+        inversion H; clear H; cleanup
+      | [H: exec' _ _ _ _ |- _ ] =>
+        inversion H; clear H; cleanup
+      end.
+    unfold refines_to in *; cleanup; eauto.
+  Qed.
 
-                              Lemma wcp_low_to_high_read :
-                                forall a,
-                                  wcp_low_to_high_prog' _ _ _ _ refinement _ (|Read a|).
-                              Proof.
-                                unfold wcp_low_to_high_prog'; simpl; intros; cleanup.
-                                unfold compilation_of in *; simpl in *; subst.
-                                split_ors; cleanup; eapply exec_deterministic_wrt_oracle in H0; eauto; cleanup.
+  
+  Lemma wp_low_to_high_commit :
+    wp_low_to_high_prog' _ _ _ _ refinement _ (|Commit|).
+  Proof.
+    unfold wp_low_to_high_prog', compilation_of; simpl; intros; cleanup.
+    unfold compilation_of in *; simpl in *; intros; cleanup.
+    split_ors; cleanup; eapply exec_deterministic_wrt_oracle in H0; eauto; cleanup.
+    eapply exec_to_sp with (P := fun o s => refines_to s s2) in H3; eauto.
+    simpl in *; cleanup.
+    eexists; intuition eauto.    
+    unfold refines_to; simpl; cleanup; eauto.
+    intuition.
+    unfold refines_to in H1; cleanup; intuition;
+    setoid_rewrite H14 in D; cleanup.
+    rewrite <- H7; eauto.
+  Qed.
 
-                                split_ors; cleanup; eauto.
-                                eexists; intuition eauto.
-                                - right; intuition eauto.
-                                  unfold refines_to in *; cleanup;
-                                  setoid_rewrite H2 in D; cleanup.
-                                  rewrite <- apply_list_get_latest_eq; eauto.
-                                - right; intuition eauto.
-                                  unfold refines_to in *; cleanup;
-                                  setoid_rewrite H2 in D; cleanup.
-                                  rewrite <- apply_list_get_latest_eq; eauto.
-                              Qed.
+  Lemma wp_high_to_low_commit :
+    wp_high_to_low_prog' _ _ _ _ refinement _ (|Commit|).
+  Proof.
+    unfold wp_high_to_low_prog', compilation_of; simpl; intros; cleanup.
+    unfold compilation_of in *; simpl; intros; cleanup.
+    repeat (split_ors; cleanup).
 
-                              Lemma wcp_high_to_low_read :
-                                forall a,
-                                  wcp_high_to_low_prog' _ _ _ _ refinement _ (|Read a|).
-                              Proof.
-                                unfold wcp_high_to_low_prog', compilation_of; simpl; intros; cleanup.
-                                unfold compilation_of in *; simpl; intros; cleanup.
-                                repeat (split_ors; cleanup);
-                                repeat invert_exec;
-                                cleanup;
-                                repeat match goal with
-                                       | [H: Operation.exec _ _ _ _ _ |- _ ] =>
-                                         inversion H; clear H; cleanup
-                                       | [H: exec' _ _ _ _ |- _ ] =>
-                                         inversion H; clear H; cleanup
-                                       end;
-                                eapply exec_to_wcp; eauto.
-                              Qed.
+    repeat invert_exec; cleanup.    
+    eapply exec_to_wp; eauto.
+    eapply exec_to_sp with (P := fun o s => refines_to s s2) in H; eauto.
+    simpl in *; cleanup.
+    eexists; intuition eauto.
+    unfold refines_to; simpl; cleanup; eauto.
+    intuition.
+    unfold refines_to in H1; cleanup; intuition;
+    setoid_rewrite H2 in D; cleanup.
+    rewrite <- H7; eauto.
+  Qed.
 
-                              Lemma wp_low_to_high_write :
-                                forall a vl,
-                                  wp_low_to_high_prog' _ _ _ _ refinement _ (|Write a vl|).
-                              Proof.
-                                unfold wp_low_to_high_prog', compilation_of; simpl; intros; cleanup.
-                                unfold compilation_of in *; simpl; intros; cleanup.
-                                split_ors; cleanup; eapply exec_deterministic_wrt_oracle in H0; eauto; cleanup.
-                                eapply exec_to_sp with (P := fun o s => refines_to s s2) in H3; eauto.
-                                unfold write in *.
-                                simpl in *; cleanup.
-                                simpl in *; cleanup.
-                                eexists; intuition eauto.
-                                clear H1 H17; unfold refines_to in *; simpl in *; cleanup.
-                                rewrite apply_list_app; eauto.
-                              Qed.
+  Lemma wcp_low_to_high_commit :
+    wcp_low_to_high_prog' _ _ _ _ refinement _ (|Commit|).
+  Proof.
+    unfold wcp_low_to_high_prog', compilation_of; simpl; intros; cleanup.
+    unfold compilation_of in *; simpl in *; intros; cleanup.
+    split_ors; cleanup; eapply exec_deterministic_wrt_oracle in H0; eauto; cleanup.
+    split_ors; cleanup; eauto.
+    eexists; intuition eauto.
+    right; intuition eauto.
+    unfold refines_to; simpl; cleanup; eauto.
+    intuition.
+    unfold refines_to in H1; cleanup; intuition;
+    setoid_rewrite H2 in D; cleanup; eauto.
+  Qed.
 
-                              Lemma wp_high_to_low_write :
-                                forall a vl,
-                                  wp_high_to_low_prog' _ _ _ _ refinement _ (|Write a vl|).
-                              Proof.
-                                unfold wp_high_to_low_prog', compilation_of; simpl; intros; cleanup.
-                                unfold compilation_of in *; simpl; intros; cleanup.
-                                repeat invert_exec; cleanup.
-                                repeat (split_ors; cleanup).
-                                eapply exec_to_wp; simpl; eauto.
-                                eapply exec_to_sp with (P := fun o s => refines_to s s2) in H; eauto.
-                                unfold write in *.
-                                simpl in *; cleanup.
-                                eexists; intuition eauto.
-                                clear H1; unfold refines_to in *; simpl in *; cleanup.
-                                rewrite apply_list_app; eauto.
-                                rewrite <- H1 at 1; rewrite apply_list_app; simpl; eauto.
-                              Qed.
+  Lemma wcp_high_to_low_commit :
+    wcp_high_to_low_prog' _ _ _ _ refinement _ (|Commit|).
+  Proof.
+    unfold wcp_high_to_low_prog', compilation_of; simpl; intros; cleanup.
+    unfold compilation_of in *; simpl in *; intros; cleanup.
+    split_ors; cleanup.
+    repeat invert_exec.
+    eapply exec_to_wcp; eauto.
+    split_ors; cleanup.
+    repeat invert_exec; eauto.
+    repeat invert_exec; eauto.
+    cleanup.
+    repeat
+      match goal with
+      | [H: Operation.exec _ _ _ _ _ |- _ ] =>
+        inversion H; clear H; cleanup
+      | [H: exec' _ _ _ _ |- _ ] =>
+        inversion H; clear H; cleanup
+      end.
+    unfold refines_to; simpl; cleanup; eauto.
+    clear H4; intuition.
+    unfold refines_to in H1; cleanup; intuition;
+    setoid_rewrite H2 in D; cleanup; eauto.
+  Qed.
+  
 
-                              
-                              Lemma wcp_low_to_high_write :
-                                forall a vl,
-                                  wcp_low_to_high_prog' _ _ _ _ refinement _ (|Write a vl|).
-                              Proof.
-                                unfold wcp_low_to_high_prog', compilation_of; simpl; intros; cleanup.
-                                unfold compilation_of in *; simpl; intros; cleanup.
-                                split_ors; cleanup; eapply exec_deterministic_wrt_oracle in H0; eauto; cleanup.
-                                split_ors; cleanup;
-                                eexists; intuition eauto.
+  Lemma wp_low_to_high_ret :
+    forall T (v: T),
+      wp_low_to_high_prog' _ _ _ _ refinement _ (Ret v).
+  Proof.
+    unfold wp_low_to_high_prog', compilation_of; simpl; intros; cleanup.
+    unfold compilation_of in *; simpl in *; intros; cleanup.
+    split_ors; cleanup; eapply exec_deterministic_wrt_oracle in H0; eauto; cleanup.
+    invert_exec; intuition eauto.
+  Qed.
 
-                                right; intuition eauto.
-                                apply refines_to_upd; eauto.
-                              Qed.
+  Lemma wp_high_to_low_ret :
+    forall T (v: T),
+      wp_high_to_low_prog' _ _ _ _ refinement _ (Ret v).
+  Proof.
+    unfold wp_high_to_low_prog', compilation_of; simpl; intros; cleanup.
+    unfold compilation_of in *; simpl; intros; cleanup.
+    split_ors; cleanup.
+    repeat invert_exec.
+    clear H4; eapply exec_to_wp; simpl; eauto.
+    econstructor.
+  Qed.
 
-                              Lemma wcp_high_to_low_write :
-                                forall a vl,
-                                  wcp_high_to_low_prog' _ _ _ _ refinement _ (|Write a vl|).
-                              Proof.
-                                unfold wcp_high_to_low_prog', compilation_of; simpl; intros; cleanup.
-                                unfold compilation_of in *; simpl; intros; cleanup.
-                                repeat split_ors; cleanup; repeat invert_exec;
-                                try inversion H8; try clear H8; cleanup;
-                                try inversion H9; try clear H9; cleanup;
-                                eapply exec_to_wcp; eauto.
-                                - split_ors; cleanup; eauto.
-                                  
-                                - split_ors; cleanup; eauto.
-                                  repeat invert_exec;
-                                  repeat match goal with
-                                         | [H: Operation.exec _ _ _ _ _ |- _ ] =>
-                                           inversion H; clear H; cleanup
-                                         | [H: exec' _ _ _ _ |- _ ] =>
-                                           inversion H; clear H; cleanup
-                                         end.
-                                  eapply refines_to_upd; eauto.
-                              Qed.
+  Lemma wcp_low_to_high_ret :
+    forall T (v: T),
+      wcp_low_to_high_prog' _ _ _ _ refinement _ (Ret v).
+  Proof.
+    unfold wcp_low_to_high_prog', compilation_of; simpl; intros; cleanup.
+    unfold compilation_of in *; simpl in *; intros; cleanup.
+    split_ors; cleanup; eapply exec_deterministic_wrt_oracle in H0; eauto; cleanup.
+    eexists; intuition eauto.
+    invert_exec; eauto.
+  Qed.
 
-                              Lemma wp_low_to_high_start :
-                                wp_low_to_high_prog' _ _ _ _ refinement _ (|Start|).
-                              Proof.
-                                unfold wp_low_to_high_prog', compilation_of; simpl; intros; cleanup.
-                                unfold compilation_of in *; simpl in *; intros; cleanup.
-                                split_ors; cleanup; eapply exec_deterministic_wrt_oracle in H0; eauto; cleanup.
-                                eapply exec_to_sp with (P := fun o s => refines_to s s2) in H3; eauto.
-                                simpl in *; cleanup.
-                                eexists; intuition eauto.
-                                clear H0 H9.
-                                unfold refines_to in *; cleanup; eauto.
-                              Qed.
+  Lemma wcp_high_to_low_ret :
+    forall T (v: T),
+      wcp_high_to_low_prog' _ _ _ _ refinement _ (Ret v).
+  Proof.
+    unfold wcp_high_to_low_prog', compilation_of; simpl; intros; cleanup.
+    unfold compilation_of in *; simpl in *; intros; cleanup.
+    split_ors; cleanup.
+    repeat invert_exec.
+    eapply exec_to_wcp; eauto.
+    econstructor; eauto.
+  Qed.
+  
+  Theorem sbs_read :
+    forall a,
+      StrongBisimulationForProgram refinement (|Read a|).              
+  Proof.
+    intros.
+    eapply bisimulation_from_wp_prog; eauto.
+    exact exec_preserves_refinement.
+    exact exec_compiled_preserves_refinement.
+    eapply Build_WP_Bisimulation_prog.
+    apply wp_low_to_high_read.
+    apply wp_high_to_low_read.    
+    apply wcp_low_to_high_read.
+    apply wcp_high_to_low_read.
+  Qed.
 
-                              Lemma wp_high_to_low_start :
-                                wp_high_to_low_prog' _ _ _ _ refinement _ (|Start|).
-                              Proof.
-                                unfold wp_high_to_low_prog', compilation_of; simpl; intros; cleanup.
-                                unfold compilation_of in *; simpl; intros; cleanup.
-                                repeat (split_ors; cleanup).
+  Theorem sbs_write :
+    forall a lv,
+      StrongBisimulationForProgram refinement (|Write a lv|).              
+  Proof.
+    intros.
+    eapply bisimulation_from_wp_prog; eauto.
+    exact exec_preserves_refinement.
+    exact exec_compiled_preserves_refinement.
+    eapply Build_WP_Bisimulation_prog.
+    apply wp_low_to_high_write.
+    apply wp_high_to_low_write.
+    apply wcp_low_to_high_write.
+    apply wcp_high_to_low_write.
+  Qed.
 
-                                repeat invert_exec; cleanup.    
-                                eapply exec_to_wp; eauto.
-                                eapply exec_to_sp with (P := fun o s => refines_to s s2) in H; eauto.
-                                simpl in *; cleanup.
-                                eexists; intuition eauto.
-                                clear H H5.
-                                unfold refines_to in *; cleanup; eauto.
-                              Qed.
+  Theorem sbs_start :
+    StrongBisimulationForProgram refinement (|Start|).              
+  Proof.
+    intros.
+    eapply bisimulation_from_wp_prog; eauto.
+    exact exec_preserves_refinement.
+    exact exec_compiled_preserves_refinement.
+    apply Build_WP_Bisimulation_prog.
+    apply wp_low_to_high_start.
+    apply wp_high_to_low_start.
+    apply wcp_low_to_high_start.
+    apply wcp_high_to_low_start.
+  Qed.
 
-                              Lemma wcp_low_to_high_start :
-                                wcp_low_to_high_prog' _ _ _ _ refinement _ (|Start|).
-                              Proof.
-                                unfold wcp_low_to_high_prog', compilation_of; simpl; intros; cleanup.
-                                unfold compilation_of in *; simpl in *; intros; cleanup.
-                                split_ors; cleanup; eapply exec_deterministic_wrt_oracle in H0; eauto; cleanup.
-                                split_ors; cleanup; eauto.
-                                eexists; intuition eauto.
-                                right; unfold refines_to in *; cleanup; eauto.
-                              Qed.
+  Theorem sbs_abort :
+    StrongBisimulationForProgram refinement (|Abort|).              
+  Proof.
+    intros.
+    eapply bisimulation_from_wp_prog; eauto.
+    exact exec_preserves_refinement.
+    exact exec_compiled_preserves_refinement.
+    apply Build_WP_Bisimulation_prog.
+    apply wp_low_to_high_abort.
+    apply wp_high_to_low_abort.
+    apply wcp_low_to_high_abort.
+    apply wcp_high_to_low_abort.
+  Qed.
 
-                              Lemma wcp_high_to_low_start :
-                                wcp_high_to_low_prog' _ _ _ _ refinement _ (|Start|).
-                              Proof.
-                                unfold wcp_high_to_low_prog', compilation_of; simpl; intros; cleanup.
-                                unfold compilation_of in *; simpl in *; intros; cleanup.
-                                split_ors; cleanup.
-                                repeat invert_exec.
-                                eapply exec_to_wcp; eauto.
-                                split_ors; cleanup.
-                                repeat invert_exec; eauto.
-                                repeat invert_exec; eauto.
-                                cleanup.
-                                repeat
-                                  match goal with
-                                  | [H: Operation.exec _ _ _ _ _ |- _ ] =>
-                                    inversion H; clear H; cleanup
-                                  | [H: exec' _ _ _ _ |- _ ] =>
-                                    inversion H; clear H; cleanup
-                                  end.
-                                unfold refines_to in *; cleanup; eauto.
-                              Qed.
+  Theorem sbs_commit :
+    StrongBisimulationForProgram refinement (|Commit|).              
+  Proof.
+    intros.
+    eapply bisimulation_from_wp_prog; eauto.
+    exact exec_preserves_refinement.
+    exact exec_compiled_preserves_refinement.
+    apply Build_WP_Bisimulation_prog.
+    apply wp_low_to_high_commit.
+    apply wp_high_to_low_commit.
+    apply wcp_low_to_high_commit.
+    apply wcp_high_to_low_commit.
+  Qed.
 
-                              
-                              Lemma wp_low_to_high_abort :
-                                wp_low_to_high_prog' _ _ _ _ refinement _ (|Abort|).
-                              Proof.
-                                unfold wp_low_to_high_prog', compilation_of; simpl; intros; cleanup.
-                                unfold compilation_of in *; simpl in *; intros; cleanup.
-                                split_ors; cleanup; eapply exec_deterministic_wrt_oracle in H0; eauto; cleanup.
-                                eapply exec_to_sp with (P := fun o s => refines_to s s2) in H3; eauto.
-                                simpl in *; cleanup.
-                                eexists; intuition eauto.
-                                clear H1 H9.
-                                unfold refines_to in *; simpl in *; cleanup; eauto.
-                              Qed.
+  
+  Theorem sbs_ret :
+    forall T (v: T),
+      StrongBisimulationForProgram refinement (Ret v).              
+  Proof.
+    intros.
+    eapply bisimulation_from_wp_prog; eauto.
+    exact exec_preserves_refinement.
+    exact exec_compiled_preserves_refinement.
+    eapply Build_WP_Bisimulation_prog.
+    apply wp_low_to_high_ret.
+    apply wp_high_to_low_ret.
+    apply wcp_low_to_high_ret.
+    apply wcp_high_to_low_ret.
+  Qed.
 
-                              Lemma wp_high_to_low_abort :
-                                wp_high_to_low_prog' _ _ _ _ refinement _ (|Abort|).
-                              Proof.
-                                unfold wp_high_to_low_prog', compilation_of; simpl; intros; cleanup.
-                                unfold compilation_of in *; simpl; intros; cleanup.
-                                repeat (split_ors; cleanup).
+  Theorem sbs_bind:
+    forall T1 T2 (p1: high.(prog) T1) (p2: T1 -> high.(prog) T2),
+      StrongBisimulationForProgram refinement p1 ->
+      (forall t, StrongBisimulationForProgram refinement (p2 t)) ->
+      StrongBisimulationForProgram refinement (Bind p1 p2).
+  Proof.
+    intros.
+    edestruct H.
+    constructor; intros.
+    simpl in *; unfold compilation_of in *;
+    simpl in *; cleanup.
 
-                                repeat invert_exec; cleanup.    
-                                eapply exec_to_wp; eauto.
-                                eapply exec_to_sp with (P := fun o s => refines_to s s2) in H; eauto.
-                                simpl in *; cleanup.
-                                eexists; intuition eauto.
-                                clear H1 H5.
-                                unfold refines_to in *; simpl; cleanup; eauto.
-                              Qed.
+    split; intros.
+    - (* Low to High *)
+      invert_exec; cleanup.
+      
+      + split_ors; cleanup.
+        eapply_fresh exec_deterministic_wrt_oracle_prefix in H5; eauto; cleanup.
+        
+        eapply_fresh exec_finished_deterministic_prefix in H5; eauto; cleanup.
+        eapply_fresh exec_deterministic_wrt_oracle in H6; eauto; cleanup.
+        edestruct strong_bisimulation_for_program_correct; eauto.
+        edestruct H2; eauto; simpl in *; cleanup; try intuition; clear H2 H3.
+        edestruct H0.
+        simpl in *; unfold compilation_of in *;
+        edestruct strong_bisimulation_for_program_correct0; eauto.
+        edestruct H2; eauto; simpl in *; cleanup; try intuition; clear H2 H3.
+        cleanup.
+        eexists; intuition eauto.
+        econstructor; eauto.
+        simpl; eauto.
+        
+      +
+        split_ors; cleanup;
+        split_ors; cleanup;
+        eapply_fresh exec_deterministic_wrt_oracle_prefix in H4; eauto; cleanup;
+        try solve [eapply_fresh exec_deterministic_wrt_oracle_prefix in H5; eauto; cleanup].
+        *
+          edestruct strong_bisimulation_for_program_correct; eauto.
+          edestruct H6; eauto; simpl in *; cleanup; try intuition; clear H6 H7.
+          exists (Crashed s); repeat (split; eauto).
+          eapply ExecBindCrash; eauto.
 
-                              Lemma wcp_low_to_high_abort :
-                                wcp_low_to_high_prog' _ _ _ _ refinement _ (|Abort|).
-                              Proof.
-                                unfold wcp_low_to_high_prog', compilation_of; simpl; intros; cleanup.
-                                unfold compilation_of in *; simpl in *; intros; cleanup.
-                                split_ors; cleanup; eapply exec_deterministic_wrt_oracle in H0; eauto; cleanup.
-                                split_ors; cleanup; eauto.
-                                eexists; intuition eauto.
-                                right; unfold refines_to in *; cleanup; eauto.
-                              Qed.
+        *
+          eapply_fresh exec_finished_deterministic_prefix in H5; eauto; cleanup.
+          eapply_fresh exec_deterministic_wrt_oracle in H6; eauto; cleanup.
+          edestruct strong_bisimulation_for_program_correct; eauto.
+          edestruct H2; eauto; simpl in *; cleanup; try intuition; clear H2 H3.
+          edestruct H0.
+          simpl in *; unfold compilation_of in *;
+          edestruct strong_bisimulation_for_program_correct0; eauto.
+          edestruct H2; eauto; simpl in *; cleanup; try intuition; clear H2 H3.
+          cleanup.
+          eexists; intuition eauto.
+          econstructor; eauto.
+          simpl; eauto.
 
-                              Lemma wcp_high_to_low_abort :
-                                wcp_high_to_low_prog' _ _ _ _ refinement _ (|Abort|).
-                              Proof.
-                                unfold wcp_high_to_low_prog', compilation_of; simpl; intros; cleanup.
-                                unfold compilation_of in *; simpl in *; intros; cleanup.
-                                split_ors; cleanup.
-                                repeat invert_exec.
-                                eapply exec_to_wcp; eauto.
-                                split_ors; cleanup.
-                                repeat invert_exec; eauto.
-                                repeat invert_exec; eauto.
-                                cleanup.
-                                repeat
-                                  match goal with
-                                  | [H: Operation.exec _ _ _ _ _ |- _ ] =>
-                                    inversion H; clear H; cleanup
-                                  | [H: exec' _ _ _ _ |- _ ] =>
-                                    inversion H; clear H; cleanup
-                                  end.
-                                unfold refines_to in *; cleanup; eauto.
-                              Qed.
+    - (* High to Low *)
+      invert_exec; cleanup.
+      
 
-                              
-                              Lemma wp_low_to_high_commit :
-                                wp_low_to_high_prog' _ _ _ _ refinement _ (|Commit|).
-                              Proof.
-                                unfold wp_low_to_high_prog', compilation_of; simpl; intros; cleanup.
-                                unfold compilation_of in *; simpl in *; intros; cleanup.
-                                split_ors; cleanup; eapply exec_deterministic_wrt_oracle in H0; eauto; cleanup.
-                                eapply exec_to_sp with (P := fun o s => refines_to s s2) in H3; eauto.
-                                simpl in *; cleanup.
-                                eexists; intuition eauto.    
-                                unfold refines_to; simpl; cleanup; eauto.
-                                intuition.
-                                unfold refines_to in H1; cleanup; intuition;
-                                setoid_rewrite H14 in D; cleanup.
-                                rewrite <- H7; eauto.
-                              Qed.
+      + split_ors; cleanup.
+        edestruct strong_bisimulation_for_program_correct; eauto.
+        edestruct H7; eauto; simpl in *; cleanup; try intuition; clear H7 H8.
+        eapply_fresh exec_deterministic_wrt_oracle_prefix in H2; eauto; cleanup.
 
-                              Lemma wp_high_to_low_commit :
-                                wp_high_to_low_prog' _ _ _ _ refinement _ (|Commit|).
-                              Proof.
-                                unfold wp_high_to_low_prog', compilation_of; simpl; intros; cleanup.
-                                unfold compilation_of in *; simpl; intros; cleanup.
-                                repeat (split_ors; cleanup).
+        edestruct strong_bisimulation_for_program_correct; eauto.
+        edestruct H9; eauto; simpl in *; cleanup; try intuition; clear H9 H10.
+        eapply_fresh exec_finished_deterministic_prefix in H2; eauto; cleanup.
+        simpl in *.
+        edestruct H0.
+        simpl in *; unfold compilation_of in *;
+        edestruct strong_bisimulation_for_program_correct0; eauto.
+        edestruct H4; eauto; simpl in *; cleanup; try intuition; clear H4 H9; cleanup.           
+        eapply_fresh exec_deterministic_wrt_oracle in H3; eauto; cleanup.
+        eexists; intuition eauto.
+        econstructor; eauto.
+        
+      +
+        split_ors; cleanup;
+        split_ors; cleanup;
+        eapply_fresh exec_deterministic_wrt_oracle_prefix in H4; eauto; cleanup;
+        try solve [eapply_fresh exec_deterministic_wrt_oracle_prefix in H5; eauto; cleanup].
+        *
+          edestruct strong_bisimulation_for_program_correct; eauto.
+          edestruct H6; eauto; simpl in *; cleanup; try intuition; clear H6 H7.
+          eapply_fresh exec_deterministic_wrt_oracle_prefix in H3; eauto; cleanup.
+          simpl in *.
+          exists (Crashed x5); repeat (split; eauto).
+          eapply ExecBindCrash; eauto.
 
-                                repeat invert_exec; cleanup.    
-                                eapply exec_to_wp; eauto.
-                                eapply exec_to_sp with (P := fun o s => refines_to s s2) in H; eauto.
-                                simpl in *; cleanup.
-                                eexists; intuition eauto.
-                                unfold refines_to; simpl; cleanup; eauto.
-                                intuition.
-                                unfold refines_to in H1; cleanup; intuition;
-                                setoid_rewrite H2 in D; cleanup.
-                                rewrite <- H7; eauto.
-                              Qed.
+        *
+          edestruct strong_bisimulation_for_program_correct; eauto.
+          edestruct H8; eauto; simpl in *; cleanup; try intuition; clear H8 H9.
+          eapply_fresh exec_deterministic_wrt_oracle_prefix in H3; eauto; cleanup.
 
-                              Lemma wcp_low_to_high_commit :
-                                wcp_low_to_high_prog' _ _ _ _ refinement _ (|Commit|).
-                              Proof.
-                                unfold wcp_low_to_high_prog', compilation_of; simpl; intros; cleanup.
-                                unfold compilation_of in *; simpl in *; intros; cleanup.
-                                split_ors; cleanup; eapply exec_deterministic_wrt_oracle in H0; eauto; cleanup.
-                                split_ors; cleanup; eauto.
-                                eexists; intuition eauto.
-                                right; intuition eauto.
-                                unfold refines_to; simpl; cleanup; eauto.
-                                intuition.
-                                unfold refines_to in H1; cleanup; intuition;
-                                setoid_rewrite H2 in D; cleanup; eauto.
-                              Qed.
+        *
+          edestruct strong_bisimulation_for_program_correct; eauto.
+          edestruct H7; eauto; simpl in *; cleanup; try intuition; clear H7 H8.
+          eapply_fresh exec_deterministic_wrt_oracle_prefix in H3; eauto; cleanup.
 
-                              Lemma wcp_high_to_low_commit :
-                                wcp_high_to_low_prog' _ _ _ _ refinement _ (|Commit|).
-                              Proof.
-                                unfold wcp_high_to_low_prog', compilation_of; simpl; intros; cleanup.
-                                unfold compilation_of in *; simpl in *; intros; cleanup.
-                                split_ors; cleanup.
-                                repeat invert_exec.
-                                eapply exec_to_wcp; eauto.
-                                split_ors; cleanup.
-                                repeat invert_exec; eauto.
-                                repeat invert_exec; eauto.
-                                cleanup.
-                                repeat
-                                  match goal with
-                                  | [H: Operation.exec _ _ _ _ _ |- _ ] =>
-                                    inversion H; clear H; cleanup
-                                  | [H: exec' _ _ _ _ |- _ ] =>
-                                    inversion H; clear H; cleanup
-                                  end.
-                                unfold refines_to; simpl; cleanup; eauto.
-                                clear H4; intuition.
-                                unfold refines_to in H1; cleanup; intuition;
-                                setoid_rewrite H2 in D; cleanup; eauto.
-                              Qed.
-                              
+        *
+          edestruct strong_bisimulation_for_program_correct; eauto.
+          edestruct H9; eauto; simpl in *; cleanup; try intuition; clear H9 H10.
+          eapply_fresh exec_finished_deterministic_prefix in H3; eauto; cleanup.
+          edestruct H0.
+          simpl in *; unfold compilation_of in *;
+          edestruct strong_bisimulation_for_program_correct0; eauto.
+          edestruct H2; eauto; simpl in *; cleanup; try intuition; clear H2 H9.
+          cleanup.
+          eapply_fresh exec_deterministic_wrt_oracle in H4; eauto; cleanup.
+          eexists; intuition eauto.
+          econstructor; eauto.
+          Unshelve.
+          all: eauto.
+  Qed.
 
-                              Lemma wp_low_to_high_ret :
-                                forall T (v: T),
-                                  wp_low_to_high_prog' _ _ _ _ refinement _ (Ret v).
-                              Proof.
-                                unfold wp_low_to_high_prog', compilation_of; simpl; intros; cleanup.
-                                unfold compilation_of in *; simpl in *; intros; cleanup.
-                                split_ors; cleanup; eapply exec_deterministic_wrt_oracle in H0; eauto; cleanup.
-                                invert_exec; intuition eauto.
-                              Qed.
+  Hint Resolve sbs_read sbs_write sbs_start sbs_abort sbs_commit sbs_ret sbs_bind : core.
+  
+  Theorem sbs :
+    StrongBisimulation refinement.              
+  Proof.
+    apply bisimulation_restrict_prog.
+    induction p; eauto.
+    destruct p; eauto.
+  Qed.
 
-                              Lemma wp_high_to_low_ret :
-                                forall T (v: T),
-                                  wp_high_to_low_prog' _ _ _ _ refinement _ (Ret v).
-                              Proof.
-                                unfold wp_high_to_low_prog', compilation_of; simpl; intros; cleanup.
-                                unfold compilation_of in *; simpl; intros; cleanup.
-                                split_ors; cleanup.
-                                repeat invert_exec.
-                                clear H4; eapply exec_to_wp; simpl; eauto.
-                                econstructor.
-                              Qed.
+  Hint Resolve sbs : core.
 
-                              Lemma wcp_low_to_high_ret :
-                                forall T (v: T),
-                                  wcp_low_to_high_prog' _ _ _ _ refinement _ (Ret v).
-                              Proof.
-                                unfold wcp_low_to_high_prog', compilation_of; simpl; intros; cleanup.
-                                unfold compilation_of in *; simpl in *; intros; cleanup.
-                                split_ors; cleanup; eapply exec_deterministic_wrt_oracle in H0; eauto; cleanup.
-                                eexists; intuition eauto.
-                                invert_exec; eauto.
-                              Qed.
+  Theorem sbs_general:
+    forall valid_state_h valid_prog_h,
+      exec_compiled_preserves_validity refinement
+                                       (refines_to_valid refinement valid_state_h) ->
+      
+      exec_preserves_validity TransactionalDiskLang valid_state_h ->
+      
+      StrongBisimulationForValidStates refinement
+                                       (refines_to_valid refinement valid_state_h)
+                                       valid_state_h
+                                       (compiles_to_valid refinement valid_prog_h)        
+                                       valid_prog_h.  
+  Proof.
+    intros.
+    eapply bisimulation_restrict_state; eauto.
+  Qed.
 
-                              Lemma wcp_high_to_low_ret :
-                                forall T (v: T),
-                                  wcp_high_to_low_prog' _ _ _ _ refinement _ (Ret v).
-                              Proof.
-                                unfold wcp_high_to_low_prog', compilation_of; simpl; intros; cleanup.
-                                unfold compilation_of in *; simpl in *; intros; cleanup.
-                                split_ors; cleanup.
-                                repeat invert_exec.
-                                eapply exec_to_wcp; eauto.
-                                econstructor; eauto.
-                              Qed.
-                              
-                              Theorem sbs_read :
-                                forall a,
-                                  StrongBisimulationForProgram refinement (|Read a|).              
-                              Proof.
-                                intros.
-                                eapply bisimulation_from_wp_prog; eauto.
-                                exact exec_preserves_refinement.
-                                exact exec_compiled_preserves_refinement.
-                                eapply Build_WP_Bisimulation_prog.
-                                apply wp_low_to_high_read.
-                                apply wp_high_to_low_read.    
-                                apply wcp_low_to_high_read.
-                                apply wcp_high_to_low_read.
-                              Qed.
+End TransactionalDiskBisimulation.
 
-                              Theorem sbs_write :
-                                forall a lv,
-                                  StrongBisimulationForProgram refinement (|Write a lv|).              
-                              Proof.
-                                intros.
-                                eapply bisimulation_from_wp_prog; eauto.
-                                exact exec_preserves_refinement.
-                                exact exec_compiled_preserves_refinement.
-                                eapply Build_WP_Bisimulation_prog.
-                                apply wp_low_to_high_write.
-                                apply wp_high_to_low_write.
-                                apply wcp_low_to_high_write.
-                                apply wcp_high_to_low_write.
-                              Qed.
+Section TransferToTransactionCache.
 
-                              Theorem sbs_start :
-                                StrongBisimulationForProgram refinement (|Start|).              
-                              Proof.
-                                intros.
-                                eapply bisimulation_from_wp_prog; eauto.
-                                exact exec_preserves_refinement.
-                                exact exec_compiled_preserves_refinement.
-                                apply Build_WP_Bisimulation_prog.
-                                apply wp_low_to_high_start.
-                                apply wp_high_to_low_start.
-                                apply wcp_low_to_high_start.
-                                apply wcp_high_to_low_start.
-                              Qed.
+  Lemma write_all_app :
+    forall V l1 l2 (l3 l4: list V) m,
+      length l1 = length l3 ->
+      (forall i, In i l1 -> m i <> None) ->
+      write_all m (l1++l2) (l3++l4) = write_all (write_all m l1 l3) l2 l4.
+  Proof.
+    induction l1; simpl in *; destruct l3; simpl in *;
+    intros; cleanup; try congruence.
+    destruct_fresh (m a); simpl in *.
+    erewrite IHl1; eauto.
+    intros; simpl.
+    unfold upd_disk.
+    destruct (addr_dec a i); subst; [rewrite upd_eq; eauto | rewrite upd_ne; eauto];
+    congruence.
+    exfalso; eapply H0; eauto.
+  Qed.
+  
+  Lemma write_all_merge_apply_list:
+    forall x6 x4 x,
+      refines_to (Some x6, x4) x ->
+      write_all x4 (map fst (rev x6)) (map snd (rev x6)) =
+      merge (apply_list empty_mem (rev x6)) x4.
+  Proof.
+    induction x6; simpl in *; intros; eauto.
+    unfold refines_to in *; simpl in *; cleanup.
+    repeat rewrite map_app; simpl in *.
+    rewrite write_all_app, apply_list_app in *; eauto; simpl in *.
+    unfold addrs_match in *.
+    destruct a, x; simpl in *.
+    erewrite IHx6; eauto.
+    unfold upd_disk.
+    extensionality a'; simpl.
+    unfold merge at 4; simpl.
+    - destruct (addr_dec a a'); subst; simpl;
+      [rewrite upd_eq; eauto
+      | rewrite upd_ne; eauto].
+      
+      + destruct_fresh (d0 a');
+        [| exfalso; eapply H1; eauto;
+           rewrite upd_eq; eauto; congruence ].
+        destruct_fresh (apply_list empty_mem (rev x6) a').
+        * edestruct merge_some_l
+            with (m2:= d0); eauto.
+          congruence.
+          cleanup.
+          pose proof H.
+          unfold merge in H; simpl.
+          rewrite D0, D in H.
+          destruct (merge (apply_list
+                             empty_mem (rev x6)) d0 a');
+          try congruence; cleanup.
+          rewrite upd_eq; eauto.
+  Admitted.
+  
+  Lemma high_oracle_exists_ok':
+    forall T p2 p1 ol sl sl',
+      (exists sh, refines_to sl sh) ->
+      low.(exec) ol sl p1 sl' ->
+      compilation_of T p1 p2 ->
+      exists oh, oracle_refines_to T sl p2 ol oh.
+  Proof.
+    unfold compilation_of;
+    induction p2; simpl; intros; cleanup.
+    - (* Start *)
+      destruct sl'.
+      {
+        eapply exec_to_sp with (P := fun o s => refines_to s x /\ o = ol /\ s = sl) in H0 as Hx; eauto.
+        simpl in *; cleanup.
+        eexists; left; do 2 eexists; intuition eauto.
+        destruct s; simpl in *.
+        unfold refines_to in *; simpl in *; intuition subst; eauto.
+      }
+      {
+        eapply exec_to_scp with (P := fun o s => refines_to s x /\ o = ol /\ s = sl) in H0 as Hx; eauto.
+        simpl in *; cleanup.
+        split_ors; cleanup; repeat (simpl in *; try split_ors; cleanup);
+        try (inversion H1; clear H1); cleanup; eauto;
+        try solve [
+              eexists; right; do 2 eexists; intuition eauto;
+              destruct s; simpl in *; cleanup; eauto ].
+      }
+    - (* Read *)
+      destruct sl'.
+      {
+        eapply exec_to_sp with (P := fun o s => refines_to s x /\ o = ol /\ s = sl) in H0 as Hx; eauto.
+        unfold read in Hx; simpl in Hx; cleanup;
+        cleanup; simpl in *; cleanup;
+        
+        eexists; left; do 2 eexists; intuition eauto;
+        destruct s; cleanup; simpl in *; cleanup; eauto.
+      }
+      {
+        eapply exec_to_scp with (P := fun o s => refines_to s x /\ o = ol /\ s = sl) in H0 as Hx; eauto.
+        unfold read in Hx; repeat (simpl in *; cleanup).
+        split_ors; cleanup; repeat (simpl in *; try split_ors; cleanup);
+        try (inversion H1; clear H1); cleanup; eauto;
+        try solve [
+              eexists; right; do 2 eexists; intuition eauto;
+              destruct s; simpl in *; cleanup; eauto ].
+        eexists; right; do 2 eexists; intuition eauto;
+        destruct s; simpl in *; cleanup; eauto.       
+      }
+    - (* Write *)
+      destruct sl'.
+      {
+        eapply exec_to_sp with (P := fun o s => refines_to s x /\ o = ol /\ s = sl) in H0 as Hx; eauto.
+        unfold write in Hx; simpl in *; cleanup;
+        cleanup; simpl in *; cleanup;      
+        try destruct s; cleanup; simpl in *; cleanup; eauto;
+        eexists; left; do 2 eexists; intuition eauto;
+        try destruct s; cleanup; simpl in *; cleanup; eauto.
+      }
+      {
+        eapply exec_to_scp with (P := fun o s => refines_to s x /\ o = ol /\ s = sl) in H0 as Hx; eauto.
+        unfold write in Hx; repeat (simpl in *; cleanup).
+        split_ors; cleanup; repeat (simpl in *; try split_ors; cleanup);
+        inversion H1; clear H1; cleanup; eauto;
+        try solve [
+              eexists; right; do 2 eexists; intuition eauto;
+              destruct s; simpl in *; cleanup; eauto ].
+        eexists; right; do 2 eexists; intuition eauto;
+        destruct s; simpl in *; cleanup; eauto.
+      }
+    - (* Commit *)
+      destruct sl'.
+      {
+        eapply exec_to_sp with (P := fun o s => refines_to s x /\ o = ol /\ s = sl) in H0 as Hx; eauto.
+        simpl in *; cleanup.
+        cleanup; simpl in *; cleanup;
+        eexists; left; do 2 eexists; intuition eauto;
+        destruct s; cleanup; simpl in *; cleanup; eauto.
+        eexists; intuition eauto.
+        rewrite <- map_fst_split, <- map_snd_split.
+        erewrite write_all_merge_apply_list; eauto.
+      }
+      {
+        eapply exec_to_scp with (P := fun o s => refines_to s x /\ o = ol /\ s = sl) in H0 as Hx; eauto.
+        simpl in *; cleanup.
+        split_ors; cleanup; repeat (simpl in *; try split_ors; cleanup);
+        try solve [
+              inversion H1; clear H1; cleanup; eauto;
+              eexists; right; do 2 eexists; intuition eauto;
+              destruct s; simpl in *; cleanup; eauto ].
+        
+        destruct s; simpl in *; cleanup; eauto.
+        eexists; right; do 2 eexists; intuition eauto.
+        admit. (* TODO: Solve this *)
 
-                              Theorem sbs_abort :
-                                StrongBisimulationForProgram refinement (|Abort|).              
-                              Proof.
-                                intros.
-                                eapply bisimulation_from_wp_prog; eauto.
-                                exact exec_preserves_refinement.
-                                exact exec_compiled_preserves_refinement.
-                                apply Build_WP_Bisimulation_prog.
-                                apply wp_low_to_high_abort.
-                                apply wp_high_to_low_abort.
-                                apply wcp_low_to_high_abort.
-                                apply wcp_high_to_low_abort.
-                              Qed.
+        inversion H1; clear H1; cleanup; eauto.
+        eexists; right; do 2 eexists; intuition eauto;
+        destruct s; simpl in *; cleanup; eauto.
+        admit. (* TODO: Solve this *)
+        
+        eexists; right; do 2 eexists; intuition eauto;
+        destruct s; simpl in *; cleanup; eauto.
+        right; intuition eauto; eexists; intuition eauto.
+        admit. (* TODO: Solve this *)       
+      }
+      
+    - (* Abort *)
+      destruct sl'.
+      {
+        eapply exec_to_sp with (P := fun o s => refines_to s x /\ o = ol /\ s = sl) in H0 as Hx; eauto.
+        simpl in *; cleanup.
+        eexists; left; do 2 eexists; intuition eauto.
+      }
+      {
+        eapply exec_to_scp with (P := fun o s => refines_to s x /\ o = ol /\ s = sl) in H0 as Hx; eauto.
+        simpl in *; cleanup.
+        split_ors; cleanup; repeat (simpl in *; try split_ors; cleanup);
+        try (inversion H1; clear H1); cleanup; eauto;
+        try solve [
+              eexists; right; do 2 eexists; intuition eauto;
+              destruct s; simpl in *; cleanup; eauto ].
+      }
+    - destruct sl'; eexists; eauto.
+    - (* Bind *)
+      invert_exec.
+      + (* Finished *)
+        edestruct IHp2; eauto.
+        eapply_fresh exec_compiled_preserves_refinement in H1; simpl in *;  eauto.
+        cleanup; simpl in *; eauto.
+        edestruct H; eauto.
+        do 5 eexists; repeat (split; eauto).
+        right; eauto.
+        do 3 eexists; repeat (split; eauto).        
+        unfold compilation_of; eauto.
+      + (* Crashed *)
+        split_ors; cleanup.
+        * (* p1 crashed *)
+          edestruct IHp2; eauto.
+          do 5 eexists; repeat (split; eauto).
+        * (* p2 Crashed *)
+          edestruct IHp2; eauto.
+          eapply_fresh exec_compiled_preserves_refinement in H1; simpl in *; eauto.
+          cleanup; simpl in *; eauto.
+          edestruct H; eauto.
+          do 5 eexists; repeat (split; eauto).
+          right; eauto.
+          do 3 eexists; repeat (split; eauto).
+          unfold compilation_of; eauto.
+          Unshelve.
+          all: constructor.
+  Admitted.
 
-                              Theorem sbs_commit :
-                                StrongBisimulationForProgram refinement (|Commit|).              
-                              Proof.
-                                intros.
-                                eapply bisimulation_from_wp_prog; eauto.
-                                exact exec_preserves_refinement.
-                                exact exec_compiled_preserves_refinement.
-                                apply Build_WP_Bisimulation_prog.
-                                apply wp_low_to_high_commit.
-                                apply wp_high_to_low_commit.
-                                apply wcp_low_to_high_commit.
-                                apply wcp_high_to_low_commit.
-                              Qed.
-
-                              
-                              Theorem sbs_ret :
-                                forall T (v: T),
-                                  StrongBisimulationForProgram refinement (Ret v).              
-                              Proof.
-                                intros.
-                                eapply bisimulation_from_wp_prog; eauto.
-                                exact exec_preserves_refinement.
-                                exact exec_compiled_preserves_refinement.
-                                eapply Build_WP_Bisimulation_prog.
-                                apply wp_low_to_high_ret.
-                                apply wp_high_to_low_ret.
-                                apply wcp_low_to_high_ret.
-                                apply wcp_high_to_low_ret.
-                              Qed.
-
-                              Theorem sbs_bind:
-                                forall T1 T2 (p1: high.(prog) T1) (p2: T1 -> high.(prog) T2),
-                                  StrongBisimulationForProgram refinement p1 ->
-                                  (forall t, StrongBisimulationForProgram refinement (p2 t)) ->
-                                  StrongBisimulationForProgram refinement (Bind p1 p2).
-                              Proof.
-                                intros.
-                                edestruct H.
-                                constructor; intros.
-                                simpl in *; unfold compilation_of in *;
-                                simpl in *; cleanup.
-
-                                split; intros.
-                                - (* Low to High *)
-                                  invert_exec; cleanup.
-                                  
-                                  + split_ors; cleanup.
-                                    eapply_fresh exec_deterministic_wrt_oracle_prefix in H5; eauto; cleanup.
-                                    
-                                    eapply_fresh exec_finished_deterministic_prefix in H5; eauto; cleanup.
-                                    eapply_fresh exec_deterministic_wrt_oracle in H6; eauto; cleanup.
-                                    edestruct strong_bisimulation_for_program_correct; eauto.
-                                    edestruct H2; eauto; simpl in *; cleanup; try intuition; clear H2 H3.
-                                    edestruct H0.
-                                    simpl in *; unfold compilation_of in *;
-                                    edestruct strong_bisimulation_for_program_correct0; eauto.
-                                    edestruct H2; eauto; simpl in *; cleanup; try intuition; clear H2 H3.
-                                    cleanup.
-                                    eexists; intuition eauto.
-                                    econstructor; eauto.
-                                    simpl; eauto.
-                                    
-                                  +
-                                    split_ors; cleanup;
-                                    split_ors; cleanup;
-                                    eapply_fresh exec_deterministic_wrt_oracle_prefix in H4; eauto; cleanup;
-                                    try solve [eapply_fresh exec_deterministic_wrt_oracle_prefix in H5; eauto; cleanup].
-                                    *
-                                      edestruct strong_bisimulation_for_program_correct; eauto.
-                                      edestruct H6; eauto; simpl in *; cleanup; try intuition; clear H6 H7.
-                                      exists (Crashed s); repeat (split; eauto).
-                                      eapply ExecBindCrash; eauto.
-
-                                    *
-                                      eapply_fresh exec_finished_deterministic_prefix in H5; eauto; cleanup.
-                                      eapply_fresh exec_deterministic_wrt_oracle in H6; eauto; cleanup.
-                                      edestruct strong_bisimulation_for_program_correct; eauto.
-                                      edestruct H2; eauto; simpl in *; cleanup; try intuition; clear H2 H3.
-                                      edestruct H0.
-                                      simpl in *; unfold compilation_of in *;
-                                      edestruct strong_bisimulation_for_program_correct0; eauto.
-                                      edestruct H2; eauto; simpl in *; cleanup; try intuition; clear H2 H3.
-                                      cleanup.
-                                      eexists; intuition eauto.
-                                      econstructor; eauto.
-                                      simpl; eauto.
-
-                                - (* High to Low *)
-                                  invert_exec; cleanup.
-                                  
-
-                                  + split_ors; cleanup.
-                                    edestruct strong_bisimulation_for_program_correct; eauto.
-                                    edestruct H7; eauto; simpl in *; cleanup; try intuition; clear H7 H8.
-                                    eapply_fresh exec_deterministic_wrt_oracle_prefix in H2; eauto; cleanup.
-
-                                    edestruct strong_bisimulation_for_program_correct; eauto.
-                                    edestruct H9; eauto; simpl in *; cleanup; try intuition; clear H9 H10.
-                                    eapply_fresh exec_finished_deterministic_prefix in H2; eauto; cleanup.
-                                    simpl in *.
-                                    edestruct H0.
-                                    simpl in *; unfold compilation_of in *;
-                                    edestruct strong_bisimulation_for_program_correct0; eauto.
-                                    edestruct H4; eauto; simpl in *; cleanup; try intuition; clear H4 H9; cleanup.           
-                                    eapply_fresh exec_deterministic_wrt_oracle in H3; eauto; cleanup.
-                                    eexists; intuition eauto.
-                                    econstructor; eauto.
-                                    
-                                  +
-                                    split_ors; cleanup;
-                                    split_ors; cleanup;
-                                    eapply_fresh exec_deterministic_wrt_oracle_prefix in H4; eauto; cleanup;
-                                    try solve [eapply_fresh exec_deterministic_wrt_oracle_prefix in H5; eauto; cleanup].
-                                    *
-                                      edestruct strong_bisimulation_for_program_correct; eauto.
-                                      edestruct H6; eauto; simpl in *; cleanup; try intuition; clear H6 H7.
-                                      eapply_fresh exec_deterministic_wrt_oracle_prefix in H3; eauto; cleanup.
-                                      simpl in *.
-                                      exists (Crashed x5); repeat (split; eauto).
-                                      eapply ExecBindCrash; eauto.
-
-                                    *
-                                      edestruct strong_bisimulation_for_program_correct; eauto.
-                                      edestruct H8; eauto; simpl in *; cleanup; try intuition; clear H8 H9.
-                                      eapply_fresh exec_deterministic_wrt_oracle_prefix in H3; eauto; cleanup.
-
-                                    *
-                                      edestruct strong_bisimulation_for_program_correct; eauto.
-                                      edestruct H7; eauto; simpl in *; cleanup; try intuition; clear H7 H8.
-                                      eapply_fresh exec_deterministic_wrt_oracle_prefix in H3; eauto; cleanup.
-
-                                    *
-                                      edestruct strong_bisimulation_for_program_correct; eauto.
-                                      edestruct H9; eauto; simpl in *; cleanup; try intuition; clear H9 H10.
-                                      eapply_fresh exec_finished_deterministic_prefix in H3; eauto; cleanup.
-                                      edestruct H0.
-                                      simpl in *; unfold compilation_of in *;
-                                      edestruct strong_bisimulation_for_program_correct0; eauto.
-                                      edestruct H2; eauto; simpl in *; cleanup; try intuition; clear H2 H9.
-                                      cleanup.
-                                      eapply_fresh exec_deterministic_wrt_oracle in H4; eauto; cleanup.
-                                      eexists; intuition eauto.
-                                      econstructor; eauto.
-                                      Unshelve.
-                                      all: eauto.
-                              Qed.
-
-                              Hint Resolve sbs_read sbs_write sbs_start sbs_abort sbs_commit sbs_ret sbs_bind : core.
-                              
-                              Theorem sbs :
-                                StrongBisimulation refinement.              
-                              Proof.
-                                apply bisimulation_restrict_prog.
-                                induction p; eauto.
-                                destruct p; eauto.
-                              Qed.
-
-                              Hint Resolve sbs : core.
-
-                              Theorem sbs_general:
-                                forall valid_state_h valid_prog_h,
-                                  exec_compiled_preserves_validity refinement
-                                                                   (refines_to_valid refinement valid_state_h) ->
-                                  
-                                  exec_preserves_validity TransactionalDiskLang valid_state_h ->
-                                  
-                                  StrongBisimulationForValidStates refinement
-                                                                   (refines_to_valid refinement valid_state_h)
-                                                                   valid_state_h
-                                                                   (compiles_to_valid refinement valid_prog_h)        
-                                                                   valid_prog_h.  
-                              Proof.
-                                intros.
-                                eapply bisimulation_restrict_state; eauto.
-                              Qed.
-
-                              End TransactionalDiskBisimulation.
-
-                              Section TransferToTransactionCache.
-
-                                Lemma write_all_app :
-                                  forall V l1 l2 (l3 l4: list V) m,
-                                    length l1 = length l3 ->
-                                    (forall i, In i l1 -> m i <> None) ->
-                                    write_all m (l1++l2) (l3++l4) = write_all (write_all m l1 l3) l2 l4.
-                                Proof.
-                                  induction l1; simpl in *; destruct l3; simpl in *;
-                                  intros; cleanup; try congruence.
-                                  destruct_fresh (m a); simpl in *.
-                                  erewrite IHl1; eauto.
-                                  intros; simpl.
-                                  unfold upd_disk.
-                                  destruct (addr_dec a i); subst; [rewrite upd_eq; eauto | rewrite upd_ne; eauto];
-                                  congruence.
-                                  exfalso; eapply H0; eauto.
-                                Qed.
-                                
-                                Lemma write_all_merge_apply_list:
-                                  forall x6 x4 x,
-                                    refines_to (Some x6, x4) x ->
-                                    write_all x4 (map fst (rev x6)) (map snd (rev x6)) =
-                                    merge (apply_list empty_mem (rev x6)) x4.
-                                Proof.
-                                  induction x6; simpl in *; intros; eauto.
-                                  unfold refines_to in *; simpl in *; cleanup.
-                                  repeat rewrite map_app; simpl in *.
-                                  rewrite write_all_app, apply_list_app in *; eauto; simpl in *.
-                                  unfold addrs_match in *.
-                                  destruct a, x; simpl in *.
-                                  erewrite IHx6; eauto.
-                                  unfold upd_disk.
-                                  extensionality a'; simpl.
-                                  unfold merge at 4; simpl.
-                                  - destruct (addr_dec a a'); subst; simpl;
-                                    [rewrite upd_eq; eauto
-                                    | rewrite upd_ne; eauto].
-                                    
-                                    + destruct_fresh (d0 a');
-                                      [| exfalso; eapply H1; eauto;
-                                         rewrite upd_eq; eauto; congruence ].
-                                      destruct_fresh (apply_list empty_mem (rev x6) a').
-                                      * edestruct merge_some_l
-                                          with (m2:= d0); eauto.
-                                        congruence.
-                                        cleanup.
-                                        pose proof H.
-                                        unfold merge in H; simpl.
-                                        rewrite D0, D in H.
-                                        destruct (merge (apply_list
-                                                           empty_mem (rev x6)) d0 a');
-                                        try congruence; cleanup.
-                                        rewrite upd_eq; eauto.
-                                Admitted.
-                                
-                                Lemma high_oracle_exists_ok':
-                                  forall T p2 p1 ol sl sl',
-                                    (exists sh, refines_to sl sh) ->
-                                    low.(exec) ol sl p1 sl' ->
-                                    compilation_of T p1 p2 ->
-                                    exists oh, oracle_refines_to T sl p2 ol oh.
-                                Proof.
-                                  unfold compilation_of;
-                                  induction p2; simpl; intros; cleanup.
-                                  - (* Start *)
-                                    destruct sl'.
-                                    {
-                                      eapply exec_to_sp with (P := fun o s => refines_to s x /\ o = ol /\ s = sl) in H0 as Hx; eauto.
-                                      simpl in *; cleanup.
-                                      eexists; left; do 2 eexists; intuition eauto.
-                                      destruct s; simpl in *.
-                                      unfold refines_to in *; simpl in *; intuition subst; eauto.
-                                    }
-                                    {
-                                      eapply exec_to_scp with (P := fun o s => refines_to s x /\ o = ol /\ s = sl) in H0 as Hx; eauto.
-                                      simpl in *; cleanup.
-                                      split_ors; cleanup; repeat (simpl in *; try split_ors; cleanup);
-                                      try (inversion H1; clear H1); cleanup; eauto;
-                                      try solve [
-                                            eexists; right; do 2 eexists; intuition eauto;
-                                            destruct s; simpl in *; cleanup; eauto ].
-                                    }
-                                  - (* Read *)
-                                    destruct sl'.
-                                    {
-                                      eapply exec_to_sp with (P := fun o s => refines_to s x /\ o = ol /\ s = sl) in H0 as Hx; eauto.
-                                      unfold read in Hx; simpl in Hx; cleanup;
-                                      cleanup; simpl in *; cleanup;
-                                      
-                                      eexists; left; do 2 eexists; intuition eauto;
-                                      destruct s; cleanup; simpl in *; cleanup; eauto.
-                                    }
-                                    {
-                                      eapply exec_to_scp with (P := fun o s => refines_to s x /\ o = ol /\ s = sl) in H0 as Hx; eauto.
-                                      unfold read in Hx; repeat (simpl in *; cleanup).
-                                      split_ors; cleanup; repeat (simpl in *; try split_ors; cleanup);
-                                      try (inversion H1; clear H1); cleanup; eauto;
-                                      try solve [
-                                            eexists; right; do 2 eexists; intuition eauto;
-                                            destruct s; simpl in *; cleanup; eauto ].
-                                      eexists; right; do 2 eexists; intuition eauto;
-                                      destruct s; simpl in *; cleanup; eauto.       
-                                    }
-                                  - (* Write *)
-                                    destruct sl'.
-                                    {
-                                      eapply exec_to_sp with (P := fun o s => refines_to s x /\ o = ol /\ s = sl) in H0 as Hx; eauto.
-                                      unfold write in Hx; simpl in *; cleanup;
-                                      cleanup; simpl in *; cleanup;      
-                                      try destruct s; cleanup; simpl in *; cleanup; eauto;
-                                      eexists; left; do 2 eexists; intuition eauto;
-                                      try destruct s; cleanup; simpl in *; cleanup; eauto.
-                                    }
-                                    {
-                                      eapply exec_to_scp with (P := fun o s => refines_to s x /\ o = ol /\ s = sl) in H0 as Hx; eauto.
-                                      unfold write in Hx; repeat (simpl in *; cleanup).
-                                      split_ors; cleanup; repeat (simpl in *; try split_ors; cleanup);
-                                      inversion H1; clear H1; cleanup; eauto;
-                                      try solve [
-                                            eexists; right; do 2 eexists; intuition eauto;
-                                            destruct s; simpl in *; cleanup; eauto ].
-                                      eexists; right; do 2 eexists; intuition eauto;
-                                      destruct s; simpl in *; cleanup; eauto.
-                                    }
-                                  - (* Commit *)
-                                    destruct sl'.
-                                    {
-                                      eapply exec_to_sp with (P := fun o s => refines_to s x /\ o = ol /\ s = sl) in H0 as Hx; eauto.
-                                      simpl in *; cleanup.
-                                      cleanup; simpl in *; cleanup;
-                                      eexists; left; do 2 eexists; intuition eauto;
-                                      destruct s; cleanup; simpl in *; cleanup; eauto.
-                                      eexists; intuition eauto.
-                                      rewrite <- map_fst_split, <- map_snd_split.
-                                      erewrite write_all_merge_apply_list; eauto.
-                                    }
-                                    {
-                                      eapply exec_to_scp with (P := fun o s => refines_to s x /\ o = ol /\ s = sl) in H0 as Hx; eauto.
-                                      simpl in *; cleanup.
-                                      split_ors; cleanup; repeat (simpl in *; try split_ors; cleanup);
-                                      try solve [
-                                            inversion H1; clear H1; cleanup; eauto;
-                                            eexists; right; do 2 eexists; intuition eauto;
-                                            destruct s; simpl in *; cleanup; eauto ].
-                                      
-                                      destruct s; simpl in *; cleanup; eauto.
-                                      eexists; right; do 2 eexists; intuition eauto.
-                                      admit. (* TODO: Solve this *)
-
-                                      inversion H1; clear H1; cleanup; eauto.
-                                      eexists; right; do 2 eexists; intuition eauto;
-                                      destruct s; simpl in *; cleanup; eauto.
-                                      admit. (* TODO: Solve this *)
-                                      
-                                      eexists; right; do 2 eexists; intuition eauto;
-                                      destruct s; simpl in *; cleanup; eauto.
-                                      right; intuition eauto; eexists; intuition eauto.
-                                      admit. (* TODO: Solve this *)       
-                                    }
-                                    
-                                  - (* Abort *)
-                                    destruct sl'.
-                                    {
-                                      eapply exec_to_sp with (P := fun o s => refines_to s x /\ o = ol /\ s = sl) in H0 as Hx; eauto.
-                                      simpl in *; cleanup.
-                                      eexists; left; do 2 eexists; intuition eauto.
-                                    }
-                                    {
-                                      eapply exec_to_scp with (P := fun o s => refines_to s x /\ o = ol /\ s = sl) in H0 as Hx; eauto.
-                                      simpl in *; cleanup.
-                                      split_ors; cleanup; repeat (simpl in *; try split_ors; cleanup);
-                                      try (inversion H1; clear H1); cleanup; eauto;
-                                      try solve [
-                                            eexists; right; do 2 eexists; intuition eauto;
-                                            destruct s; simpl in *; cleanup; eauto ].
-                                    }
-                                  - destruct sl'; eexists; eauto.
-                                  - (* Bind *)
-                                    invert_exec.
-                                    + (* Finished *)
-                                      edestruct IHp2; eauto.
-                                      eapply_fresh exec_compiled_preserves_refinement in H1; simpl in *;  eauto.
-                                      cleanup; simpl in *; eauto.
-                                      edestruct H; eauto.
-                                      do 5 eexists; repeat (split; eauto).
-                                      right; eauto.
-                                      do 3 eexists; repeat (split; eauto).        
-                                      unfold compilation_of; eauto.
-                                    + (* Crashed *)
-                                      split_ors; cleanup.
-                                      * (* p1 crashed *)
-                                        edestruct IHp2; eauto.
-                                        do 5 eexists; repeat (split; eauto).
-                                      * (* p2 Crashed *)
-                                        edestruct IHp2; eauto.
-                                        eapply_fresh exec_compiled_preserves_refinement in H1; simpl in *; eauto.
-                                        cleanup; simpl in *; eauto.
-                                        edestruct H; eauto.
-                                        do 5 eexists; repeat (split; eauto).
-                                        right; eauto.
-                                        do 3 eexists; repeat (split; eauto).
-                                        unfold compilation_of; eauto.
-                                        Unshelve.
-                                        all: constructor.
-                                Admitted.
-
-                                Lemma high_oracle_exists_ok :
-                                  high_oracle_exists refinement. 
-                                Proof.
-                                  unfold high_oracle_exists; intros.
-                                  eapply high_oracle_exists_ok'; eauto.
-                                Qed.
+  Lemma high_oracle_exists_ok :
+    high_oracle_exists refinement. 
+  Proof.
+    unfold high_oracle_exists; intros.
+    eapply high_oracle_exists_ok'; eauto.
+  Qed.
 
 
-                                Theorem transfer_to_TransactionCache:
-                                  forall related_states_h
-                                         valid_state_h
-                                         valid_prog_h,
-                                    
-                                    SelfSimulation
-                                      high
-                                      valid_state_h
-                                      valid_prog_h
-                                      related_states_h ->
-                                    
-                                    oracle_refines_to_same_from_related refinement related_states_h ->
+  Theorem transfer_to_TransactionCache:
+    forall related_states_h
+           valid_state_h
+           valid_prog_h,
+      
+      SelfSimulation
+        high
+        valid_state_h
+        valid_prog_h
+        related_states_h ->
+      
+      oracle_refines_to_same_from_related refinement related_states_h ->
 
-                                    exec_compiled_preserves_validity refinement                           
-                                                                     (refines_to_valid refinement valid_state_h) ->
-                                    
-                                    SelfSimulation
-                                      low
-                                      (refines_to_valid refinement valid_state_h)
-                                      (compiles_to_valid refinement valid_prog_h)
-                                      (refines_to_related refinement related_states_h).
-                                Proof.
-                                  intros; eapply transfer_high_to_low; eauto.
-                                  apply sbs.
-                                  apply high_oracle_exists_ok.
-                                Qed.
+      exec_compiled_preserves_validity refinement                           
+                                       (refines_to_valid refinement valid_state_h) ->
+      
+      SelfSimulation
+        low
+        (refines_to_valid refinement valid_state_h)
+        (compiles_to_valid refinement valid_prog_h)
+        (refines_to_related refinement related_states_h).
+  Proof.
+    intros; eapply transfer_high_to_low; eauto.
+    apply sbs.
+    apply high_oracle_exists_ok.
+  Qed.
 
-                              End TransferToTransactionCache.
+End TransferToTransactionCache.
